templates/multicopy/general_multicopy_new.v
@@ -36,6 +36,13 @@ Definition traverse : val :=
   rec: "t_rec" "n" "k" :=
     lockNode "n" ;;
     let: "t" := inContents "n" "k" in
+    match: "t" with
+      SOME "t" => unlockNode "n";;
+                  "t"
+    | NONE => match: (findNext "n" "k") with
+                SOME "n'" => unlockNode "n" ;; "t_rec" "n'" "k"
+              | NONE => unlockNode "n" ;; #0 end end.
+(*              
     if: ("t" ≠ #0) 
     then
       unlockNode "n";; "t"
@@ -43,6 +50,7 @@ Definition traverse : val :=
       match: (findNext "n" "k") with
         SOME "n'" => unlockNode "n" ;; "t_rec" "n'" "k"
       | NONE => unlockNode "n" ;; #0 end.
+*)
               
 Definition search (r: Node) : val := 
   λ: "k", traverse #r "k".
@@ -159,6 +167,10 @@ Section multicopy.
 
   Definition inflow_zero (I: KT_flowint_ur K) := ∀ n, inset_KT I n = ∅. 
 
+  Definition outflow_zero (I: KT_flowint_ur K) := out_map I = ∅. 
+
+  Definition outflow_zero_R (I: inset_flowint_ur K) := out_map I = ∅. 
+
   Definition inflow_R (R: inset_flowint_ur K) r := 
     ∀ n k, if n =? r then in_inset K k R n else ¬ in_inset K k R n. 
 
@@ -168,10 +180,10 @@ Section multicopy.
   Definition outflow_constraint_I (In: KT_flowint_ur K) (es: esT) 
                           (Qn: gmap K natUR) := 
     ∀ n' k t, (k,t) ∈ outset_KT In n' ↔ 
-                          k ∈ es !!! n' ∧ (Qn !!! k = t).
+                          k ∈ es !!! n' ∧ (Qn !! k = Some t).
                           
   Definition outflow_constraint_R (Rn: inset_flowint_ur K) (es: esT) n := 
-    ∀ n' k, in_outset K k Rn n' ↔ k ∈ es !!! n' ∧ in_inset K k Rn n.
+    ∀ n' k, k ∈ outset K Rn n' ↔ k ∈ es !!! n' ∧ k ∈ inset K Rn n.
 
   Definition map_of_set (C: gset KT) : gmap K nat := 
               let f := λ (kt: KT) (M: gmap K nat), if (M !!! kt.1 <=? kt.2) 
@@ -182,42 +194,51 @@ Section multicopy.
              let f := λ k t H, H ∪ {[(k,t)]} in
              map_fold f (∅: gset KT) C.
 
-(*
-  Definition φ0 (Bn: gmap K natUR) (T: nat) := 
-              ∀ k, Bn !!! k ≤ T.  
-*)
-
   Definition φ0 (es: esT) (Qn: gmap K natUR) :=
-              ∀ k, (∀ n', k ∉ es !!! n') → Qn !!! k = 0.
+              ∀ k, (∀ n', k ∉ es !!! n') → Qn !! k = None.
 
   Definition φ1 (Bn Cn Qn: gmap K natUR) := 
-              ∀ k, (Cn !!! k > 0 → Bn !!! k = Cn !!! k)
-                 ∧ (Cn !!! k = 0 → Bn !!! k = Qn !!! k). 
+              ∀ k t, (Cn !! k = Some t → Bn !! k = Some t)
+                 ∧ (Cn !! k = None → Bn !! k = Qn !! k). 
 
-  Definition φ2 r n (Bn: gmap K natUR) In := 
-              ∀ k t, n ≠ r → (k,t) ∈ inset_KT In n → Bn !!! k = t.
+  Definition φ2 n (Bn: gmap K natUR) In := 
+              ∀ k t, (k,t) ∈ inset_KT In n → Bn !!! k = t.
 
   Definition φ3 n (Bn: gmap K natUR) Rn :=
-              ∀ k, Bn !!! k = 0 ∨ in_inset K k Rn n.
+              ∀ k, Bn !! k = None ∨ k ∈ inset K Rn n.
 
   Definition φ4 n (Rn: inset_flowint_ur K) := 
               ∀ k, inf Rn n !1 k ≤ 1.
   
-  Definition φ5 (es: esT) r :=
-                es !!! r = ∅.            
+  Definition φ5 (Bn Qn: gmap K natUR) :=
+              ∀ k, Qn !!! k ≤ Bn !!! k.            
 
   Definition φ6 (Bn: gmap K natUR) (t: nat) := 
-              ∀ k, Bn !!! k ≤ t.  
+              ∀ k, Bn !!! k ≤ t.
+  
+  Definition φ7 n (es: esT) (Rn: inset_flowint_ur K) (Qn: gmap K natUR) :=
+              ∀ k, (∃ n', k ∈ es !!! n') ∧ k ∈ inset K Rn n 
+                          → k ∈ dom (gset K) Qn.              
 
   Definition maxTS (t: nat) (H: gset KT) := 
               (∀ (k: K) t', (k, t') ∈ H → t' < t) ∧ (t > 0).
   
+  Definition f_merge (Cn: gmap K nat) (Es: gset K) (Cm: gmap K nat) := 
+                    λ k o1 o2, 
+                      if (decide (Cn !! k ≠ None)) then o1
+                      else if (decide (k ∈ Es)) then o2 
+                           else (None: option nat).
+  
+  Instance f_merge_diag_none Cn Es Cm k : DiagNone (f_merge Cn Es Cm k).
+  Proof.
+    unfold DiagNone. unfold f_merge.
+    destruct (decide (Cn !! k ≠ None)); try by simpl.
+    destruct (decide (k ∈ Es)); try by simpl.
+  Qed.  
+  
   Definition merge (Cn: gmap K nat) (Es: gset K) (Cm: gmap K nat) 
                           : (gmap K nat) :=
-             let f := λ k o1 o2, if (decide (Cn !!! k ≠ 0)) then Cn !! k
-                                 else if (decide (k ∈ Es)) then Cm !! k 
-                                      else None in
-             gmap_imerge f Cn Cm.            
+             gmap_imerge (f_merge Cn Es Cm) Cn Cm.            
 
   Definition MCS_auth (γ_te γ_he: gname) (t: nat) (H: gset KT) : iProp := 
       own γ_te (● Excl' t) ∗ own γ_he (● Excl' H).
@@ -225,7 +246,7 @@ Section multicopy.
   Definition MCS (γ_te γ_he: gname) (t: nat) (H: gset KT) : iProp := 
       own γ_te (◯ Excl' t) ∗ own γ_he (◯ Excl' H).
 
-  Definition frac_ghost_state γ_en γ_cn γ_bn γ_qn (n: Node) es 
+  Definition frac_ghost_state γ_en γ_cn γ_bn γ_qn es 
                                   (Cn Bn Qn: gmap K natUR): iProp :=
       own (γ_en) (to_frac_agree (1/2) (es))
     ∗ own (γ_cn) (to_frac_agree (1/2) (Cn))
@@ -246,7 +267,7 @@ Section multicopy.
 
   Definition clock lc (t: nat) : iProp := lc ↦ #t.
   
-  Definition history_init (H: gset KT) : iProp := ⌜∀ k, k ∈ KS → (k, 0) ∈ H⌝.
+  Definition history_init (H: gset KT) := ∀ k, k ∈ KS → (k, 0) ∈ H.
 
   Definition ghost_loc γ_en γ_cn γ_bn γ_qn (γ_cirn: gmap K gnameO) : per_node_gl := 
         to_agree (γ_en, γ_cn, γ_bn, γ_qn, γ_cirn).
@@ -255,7 +276,7 @@ Section multicopy.
     ∃ γ_en γ_cn γ_bn γ_qn γ_cirn es t,
       node r n es Cn
     ∗ own γ_gh (◯ {[n := ghost_loc γ_en γ_cn γ_bn γ_qn γ_cirn]})  
-    ∗ frac_ghost_state γ_en γ_cn γ_bn γ_qn n es Cn Bn Qn
+    ∗ frac_ghost_state γ_en γ_cn γ_bn γ_qn es Cn Bn Qn
     ∗ own γ_s (◯ set_of_map Cn)
     ∗ (if (n =? r) then own γ_t (●{1/2} MaxNat t) ∗ clock lc t else ⌜True⌝)%I.
 
@@ -263,25 +284,24 @@ Section multicopy.
           (Cn Bn Qn : gmap K natUR) H t: iProp :=
     ∃ γ_en γ_cn γ_bn γ_qn γ_cirn es In Rn,
       own γ_gh (◯ {[n := ghost_loc γ_en γ_cn γ_bn γ_qn γ_cirn]})
-    ∗ ⌜dom (gset K) γ_cirn = KS⌝                          
-    ∗ frac_ghost_state γ_en γ_cn γ_bn γ_qn n es Cn Bn Qn  
+    ∗ frac_ghost_state γ_en γ_cn γ_bn γ_qn es Cn Bn Qn  
     ∗ singleton_interfaces_ghost_state γ_I γ_R n In Rn 
     ∗ inFP γ_f n
     ∗ closed γ_f es
     ∗ outflow_constraints n In Rn es Qn
-    ∗ (if (n =? r) then ⌜Bn = map_of_set H⌝ else True)%I
+    ∗ (if (n =? r) then ⌜Bn = map_of_set H⌝ ∗ ⌜inflow_zero In⌝ else True)%I
     ∗ ([∗ set] k ∈ KS, own (γ_cirn !!! (k)) (● (MaxNat (Bn !!! k))))
-    ∗ ⌜φ0 es Qn⌝ ∗ ⌜φ1 Bn Cn Qn⌝ ∗ ⌜φ2 r n Bn In⌝ 
-    ∗ ⌜φ3 n Bn Rn⌝ ∗ ⌜φ4 n Rn⌝ ∗ ⌜φ5 es r⌝ ∗ ⌜φ6 Bn t⌝. 
+    ∗ ⌜φ0 es Qn⌝ ∗ ⌜φ1 Bn Cn Qn⌝ ∗ ⌜φ2 n Bn In⌝ ∗ ⌜φ3 n Bn Rn⌝ 
+    ∗ ⌜φ4 n Rn⌝ ∗ ⌜φ5 Bn Qn⌝ ∗ ⌜φ6 Bn t⌝ ∗ ⌜φ7 n es Rn Qn⌝. 
 
   Definition global_state γ_te γ_he γ_s γ_t γ_I γ_R γ_f γ_gh r t H 
           (hγ: gmap Node per_node_gl) (I: KT_flowint_ur K) 
           (R: inset_flowint_ur K) : iProp :=
       MCS_auth γ_te γ_he t H
-    ∗ own γ_s (● H) ∗ (history_init H)
+    ∗ own γ_s (● H) ∗ ⌜history_init H⌝
     ∗ own γ_t (●{1/2} MaxNat t)
-    ∗ own γ_I (● I)
-    ∗ own γ_R (● R) ∗ ⌜inflow_R R r⌝
+    ∗ own γ_I (● I) ∗ ⌜outflow_zero I⌝
+    ∗ own γ_R (● R) ∗ ⌜outflow_zero_R R⌝ ∗ ⌜inflow_R R r⌝
     ∗ own γ_f (● domm I)
     ∗ own γ_gh (● hγ)
     ∗ inFP γ_f r
@@ -327,7 +347,9 @@ Section multicopy.
   Parameter inContents_spec : ∀ r n es (Cn: gmap K natUR) (k: K),
      ⊢ ({{{ node r n es Cn }}}
            inContents #n #k
-       {{{ (t: nat), RET #t; node r n es Cn ∗ ⌜Cn !!! k = t⌝ }}})%I.
+       {{{ (t: option nat), 
+              RET (match t with Some t => SOMEV #t | None => NONEV end);
+                  node r n es Cn ∗ ⌜Cn !! k = t⌝ }}})%I.
 
   Parameter findNext_spec : ∀ r n es (Cn: gmap K natUR) (k: K),
      ⊢ ({{{ node r n es Cn }}}
@@ -404,9 +426,16 @@ Section multicopy.
            node r n esn Cn' ∗ node r m esm Cm' 
            ∗ ⌜set_of_map Cn' ⊆ set_of_map Cn⌝
            ∗ ⌜set_of_map Cm' ⊆ set_of_map Cn ∪ set_of_map Cm⌝
+           ∗ ⌜set_of_map Cn ∩ set_of_map Cm' ## set_of_map Cn'⌝
            ∗ ⌜merge Cn (esn !!! m) Cm = merge Cn' (esn !!! m) Cm'⌝ }}})%I.
 
   (** Useful lemmas and definitions **)
+
+  Instance test r n γ_t lc T : Laterable (if n =? r then 
+                          own γ_t (●{1 / 2} MaxNat T) ∗ clock lc T else ⌜True⌝)%I.
+  Proof.
+    destruct (n =? r); apply timeless_laterable; apply _.
+  Qed.
 
   Lemma inFP_domm γ_f n D : inFP γ_f n -∗ own γ_f (● D) -∗ ⌜n ∈ D⌝.
   Proof.
@@ -419,6 +448,31 @@ Section multicopy.
     iPureIntro. set_solver.
   Qed.
 
+  Lemma own_alloc_set (S: gset K): True ==∗ 
+          ∃ (γ: gmap K gname), ([∗ set] k ∈ S, own (γ !!! k) (● (MaxNat 0))).
+  Proof.
+    iIntros "_".
+    iInduction S as [| s S] "IH" using set_ind_L.
+    - iModIntro. iExists _. try done.
+    - iMod (own_alloc (● (MaxNat 0))) as (γs)"H'".
+      { rewrite auth_auth_valid. try done. }
+      iDestruct "IH" as ">IH".
+      iDestruct "IH" as (γ)"IH". 
+      iModIntro. iExists (<[s := γs]> γ).
+      rewrite (big_sepS_delete _ ({[s]} ∪ S) s); last by set_solver.
+      iSplitL "H'". by rewrite lookup_total_insert.
+      assert (({[s]} ∪ S) ∖ {[s]} = S) as HS. set_solver.
+      rewrite HS. 
+      iApply (big_sepS_mono 
+                  (λ y, own (γ !!! y) (● {| max_nat_car := 0 |}) )%I
+                  (λ y, own (<[s:=γs]> γ !!! y) (● {| max_nat_car := 0 |}))%I
+                  S); try done.
+      intros k k_in_S. iFrame. iIntros "H'".
+      rewrite lookup_total_insert_ne; last by set_solver. 
+      done.
+      (* No idea what is happening here *) 
+      Unshelve. exact (∅: gmap K gname).
+  Qed.
 
   Lemma ghost_heap_sync γ_gh n γ_en γ_cn γ_bn γ_qn γ_cirn 
                                       γ_en' γ_cn' γ_bn' γ_qn' γ_cirn' : 
@@ -438,9 +492,29 @@ Section multicopy.
     by iPureIntro.
   Qed.
 
-  Lemma frac_eq γ_e γ_c γ_b γ_q n es Cn Bn Qn es' Cn' Bn' Qn' : 
-              frac_ghost_state γ_e γ_c γ_b γ_q n es Cn Bn Qn -∗
-                  frac_ghost_state γ_e γ_c γ_b γ_q n es' Cn' Bn' Qn' -∗ 
+  Lemma ghost_heap_update γ_gh (hγ: gmap Node per_node_gl) n 
+                                γ_en γ_cn γ_bn γ_qn γ_cirn :
+    ⌜n ∉ dom (gset Node) hγ⌝ -∗ 
+          own γ_gh (● hγ) ==∗ 
+            own γ_gh (● <[n := ghost_loc γ_en γ_cn γ_bn γ_qn γ_cirn]> hγ)
+          ∗ own γ_gh (◯ {[n := ghost_loc γ_en γ_cn γ_bn γ_qn γ_cirn]}).
+  Proof.
+    iIntros "%". rename H into n_notin_hγ.
+    iIntros "Hown". set (<[ n := ghost_loc γ_en γ_cn γ_bn γ_qn γ_cirn ]> hγ) as hγ'.
+    iDestruct (own_update _ _ 
+        (● hγ' ⋅ ◯ {[ n := ghost_loc γ_en γ_cn γ_bn γ_qn γ_cirn ]})
+               with "Hown") as "Hown".
+    { apply auth_update_alloc. 
+      rewrite /hγ'.
+      apply alloc_local_update; last done.
+      by rewrite <-not_elem_of_dom. }
+    iMod (own_op with "Hown") as "[Ht● Ht◯]".
+    iModIntro. iFrame.
+  Qed.    
+
+  Lemma frac_eq γ_e γ_c γ_b γ_q es Cn Bn Qn es' Cn' Bn' Qn' : 
+              frac_ghost_state γ_e γ_c γ_b γ_q es Cn Bn Qn -∗
+                  frac_ghost_state γ_e γ_c γ_b γ_q es' Cn' Bn' Qn' -∗ 
                     ⌜es = es'⌝ ∗ ⌜Cn = Cn'⌝ ∗ ⌜Bn = Bn'⌝ ∗ ⌜Qn = Qn'⌝.
   Proof.
     iIntros "H1 H2". unfold frac_ghost_state.
@@ -463,11 +537,11 @@ Section multicopy.
     iPureIntro. repeat split; try done.   
   Qed.
 
-  Lemma frac_update γ_e γ_c γ_b γ_q n es Cn Bn Qn es' Cn' Bn' Qn' : 
-              frac_ghost_state γ_e γ_c γ_b γ_q n es Cn Bn Qn ∗ 
-                 frac_ghost_state γ_e γ_c γ_b γ_q n es Cn Bn Qn ==∗ 
-                      frac_ghost_state γ_e γ_c γ_b γ_q n es' Cn' Bn' Qn' ∗ 
-                        frac_ghost_state γ_e γ_c γ_b γ_q n es' Cn' Bn' Qn'.
+  Lemma frac_update γ_e γ_c γ_b γ_q es Cn Bn Qn es' Cn' Bn' Qn' : 
+              frac_ghost_state γ_e γ_c γ_b γ_q es Cn Bn Qn ∗ 
+                 frac_ghost_state γ_e γ_c γ_b γ_q es Cn Bn Qn ==∗ 
+                      frac_ghost_state γ_e γ_c γ_b γ_q es' Cn' Bn' Qn' ∗ 
+                        frac_ghost_state γ_e γ_c γ_b γ_q es' Cn' Bn' Qn'.
   Proof.
     iIntros "(H1 & H2)". 
     iDestruct "H1" as "(H1_es & H1_c & H1_b & H1_q)".
@@ -556,6 +630,12 @@ Section multicopy.
     { admit. }  
     (* { apply view_update, option_local_update, exclusive_local_update. } *)
     done.
+  Admitted.
+
+  Lemma set_of_map_member_ne (C: gmap K nat) k :
+            C !! k = None →    
+              ∀ t, (k, t) ∉ set_of_map C.
+  Proof.
   Admitted.
 
   Lemma set_of_map_member (C: gmap K nat) k t :
@@ -735,7 +815,1536 @@ Section multicopy.
       by rewrite Hc.
   Qed. 
 
+  Lemma flowint_update_result γ I I_n I_n' x :
+    ⌜flowint_update_P (KT_multiset K) I I_n I_n' x⌝ ∗ own γ x -∗
+    ∃ I', ⌜contextualLeq (KT_multiset K) I I'⌝
+          ∗ ⌜∃ I_o, I = I_n ⋅ I_o ∧ I' = I_n' ⋅ I_o⌝
+          ∗ own γ (● I' ⋅ ◯ I_n').
+  Proof.
+    unfold flowint_update_P.
+    case_eq (view_auth_proj x); last first.
+    - intros Hx. iIntros "(% & ?)". iExFalso. done.
+    - intros [q a] Hx.
+      iIntros "[HI' Hown]". iDestruct "HI'" as %HI'.
+      destruct HI' as [I' HI'].
+      destruct HI' as [Hagree [Hq [HIn [Hcontxl HIo]]]].
+      iExists I'.
+      iSplit. by iPureIntro.
+      iSplit. by iPureIntro. destruct x.
+      simpl in Hx. simpl in HIn.
+      rewrite Hx. rewrite <-HIn.
+      rewrite Hq Hagree.
+      assert (● I' ⋅ ◯ I_n' = View (Some (1%Qp, to_agree I')) I_n') as H'.
+      { rewrite /(● I' ⋅ ◯ I_n'). unfold cmra_op.
+        simpl. unfold view_op. simpl.
+        assert (ε ⋅ I_n' = I_n') as H'. by rewrite left_id.
+        rewrite H'. unfold op, cmra_op. by simpl. }   
+      by iEval (rewrite H').
+  Qed.
+
+  Lemma flowint_update_result' γ I I_n I_n' x :
+    ⌜flowint_update_P (K_multiset) I I_n I_n' x⌝ ∗ own γ x -∗
+    ∃ I', ⌜contextualLeq (K_multiset) I I'⌝
+          ∗ ⌜∃ I_o, I = I_n ⋅ I_o ∧ I' = I_n' ⋅ I_o⌝
+          ∗ own γ (● I' ⋅ ◯ I_n').
+  Proof.
+  Admitted.
+
+  Lemma dom_lookup (C: gmap K nat) k :
+        C !! k ≠ None → k ∈ dom (gset K) C.
+  Proof.
+  Admitted.
+  
+  Lemma contents_in_reach_bigS_update (S : gset K) (γ: gmap K gname) 
+                                          (Bm Bm': gmap K nat) :
+        ⌜∀ k, k ∈ S → Bm !!! k ≤ Bm' !!! k⌝ -∗ 
+          [∗ set] k ∈ S, own (γ !!! k) (● (MaxNat (Bm !!! k))) -∗
+            |==>  [∗ set] k ∈ S, own (γ !!! k) (● (MaxNat (Bm' !!! k))).
+  Proof.
+  Admitted.
+  
+  Definition map_subset (S: gset K) (C: gmap K nat) :=
+              let f := λ a s', s' ∪ {[(a, C !!! a)]} in
+                        set_fold f (∅: gset KT) S.          
+
+  Definition map_restriction (S: gset K) (C: gmap K nat) := 
+              let f := λ a m, <[a := C !!! a ]> m in
+                        set_fold f (∅: gmap K nat) S.
+                        
+  Definition set_diffval (C1 C2: gmap K nat) :=
+              let P := λ a, C1 !! a ≠ C1 !! a in
+                filter P (dom (gset K) C1 ∪ dom (gset K) C2).
+
+  Lemma flowint_insert_set_eq_KT (I1 I1' I2 I2': KT_flowint_ur K) n S :
+        I1' = outflow_insert_set_KT I1 n S →
+          I2' = inflow_insert_set_KT I2 n S →
+             I1 ⋅ I2 = I1' ⋅ I2'.
+  Proof.
+  Admitted.
+
+  Lemma flowint_delete_set_eq_KT (I1 I1' I2 I2': KT_flowint_ur K) n S :
+        I1' = outflow_delete_set_KT I1 n S →
+          I2' = inflow_delete_set_KT I2 n S →
+             I1 ⋅ I2 = I1' ⋅ I2'.
+  Proof.
+  Admitted.
+
+  Lemma flowint_insert_set_eq_K (I1 I1' I2 I2': inset_flowint_ur K) n S :
+        I1' = outflow_insert_set_K I1 n S →
+          I2' = inflow_insert_set_K I2 n S →
+             I1 ⋅ I2 = I1' ⋅ I2'.
+  Proof.
+  Admitted.
+
+
   (** Proofs **)  
+
+  Lemma compact_spec γ_te γ_he γ_s γ_t γ_I γ_R γ_f γ_gh lc r (n: Node) :
+    ⊢ mcs_inv γ_te γ_he γ_s γ_t γ_I γ_R γ_f γ_gh lc r -∗
+        inFP γ_f n -∗ <<< ∀ t H, MCS γ_te γ_he t H >>> 
+                            compact #n @ ⊤ ∖ ↑N
+                      <<< MCS γ_te γ_he t H, RET #() >>>.
+  Proof.
+    iIntros "#HInv". iLöb as "IH" forall (n).
+    iIntros "#FP_n". iIntros (Φ) "AU". wp_lam.
+    awp_apply lockNode_spec_high; try done.
+    iAaccIntro with ""; try eauto with iFrame.
+    iIntros (Cn Bn Qn)"HnP_n". iModIntro.
+    wp_pures. iDestruct "HnP_n" as (γ_en γ_cn γ_bn γ_qn γ_cirn esn T)"(node_n   
+                            & HnP_gh & HnP_frac & HnP_C & HnP_t)".
+    iPoseProof ((node_edgeset_disjoint r n) with "[$node_n]") as "%".
+    rename H into Disj_esn.                        
+    wp_apply (atCapacity_spec with "node_n").
+    iIntros (b) "(node_n & _)". destruct b; last first; wp_pures.
+    - awp_apply (unlockNode_spec_high with "[] [] [-AU]"); try done.
+      iExists γ_en, γ_cn, γ_bn, γ_qn, γ_cirn, esn, T. iFrame.
+      iAaccIntro with ""; try eauto with iFrame.
+      iIntros "_". iMod "AU" as (t H)"[MCS [_ Hclose]]".
+      iMod ("Hclose" with "MCS") as "HΦ".
+      by iModIntro.
+    - wp_apply (chooseNext_spec with "node_n").
+      iIntros (m esn' esm0 Cm0)"(node_n & es_ne & Hor)".
+      iDestruct "es_ne" as %es_ne.
+      iDestruct "Hor" as "[ Hesn' | 
+                      (Hesn' & node_m & Hl_m & Hcm & Hesm) ]"; last first.
+      + iDestruct "Hesn'" as %Hesn'.
+        iDestruct "Hcm" as %Hcm.
+        iDestruct "Hesm" as %Hesm.
+        wp_pures.
+        iApply fupd_wp. iInv "HInv" as ">H".
+        iDestruct "H" as (T0' H0 hγ0 I0 R0) "(Hglob & Hstar)".
+        iDestruct "Hglob" as "(MCS_auth & HH & Hist & Ht & HI & Out_I & HR 
+            & Out_R & Inf_R & Hf & Hγ & FP_r & Max_ts & domm_IR & domm_Iγ)".
+        iAssert (⌜m ∉ domm I0⌝)%I as "%".
+        { destruct (decide (m ∈ domm I0)); try done.
+          rewrite (big_sepS_delete _ (domm I0) m); last by eauto.
+          iDestruct "Hstar" as "(Hm & _)".
+          iDestruct "Hm" as (bm Cm Bm Qm)"(Hl_m' & _)".
+          iDestruct (mapsto_valid_2 with "Hl_m Hl_m'") as "%".
+          exfalso. done. }
+
+        iAssert (⌜n ∈ domm I0⌝)%I as "%". 
+        { by iPoseProof (inFP_domm _ _ _ with "[$FP_n] [$Hf]") as "H'". }
+        rename H into m_notin_I0. rename H1 into n_in_I0.  
+        rewrite (big_sepS_delete _ (domm I0) n); last by eauto.
+        iDestruct "Hstar" as "(H_n & Hstar')".
+        iDestruct "H_n" as (bn Cn' Bn' Qn')"(Hl_n & Hlif_n & HnS_n)".
+        iDestruct "HnS_n" as (γ_en' γ_cn' γ_bn' γ_qn' γ_cirn' es' In0 Rn0) 
+                      "(HnS_gh & HnS_frac & HnS_si & HnS_FP 
+                                & HnS_cl & HnS_oc & HnS_H & HnS_star & Hφ)".
+        iPoseProof (ghost_heap_sync with "[$HnP_gh] [$HnS_gh]") 
+                                  as "(% & % & % & % & %)".
+        subst γ_en'. subst γ_cn'. subst γ_bn'. subst γ_qn'. subst γ_cirn'.
+        iPoseProof (frac_eq with "[$HnP_frac] [$HnS_frac]") as "%".
+        destruct H as [Hes [Hc [Hb Hq]]]. 
+        subst es'. subst Cn'. subst Bn'. subst Qn'.
+          
+        set (Qm0 := ∅ : gmap K nat).  
+        set (Bm0 := ∅ : gmap K nat).  
+        set (Im0 := int {| infR := {[m := ∅]} ; outR := ∅|} : KT_flowint_ur K).
+        set (Rm0 := int {| infR := {[m := ∅]} ; outR := ∅|} : inset_flowint_ur K).
+
+        iAssert (⌜r ∈ domm I0⌝)%I as "%". 
+        { by iPoseProof (inFP_domm _ _ _ with "[$FP_r] [$Hf]") as "H'". }
+        rename H into r_in_I0.
+        assert (m ≠ r) as m_neq_r. 
+        { clear -m_notin_I0 r_in_I0. set_solver. }
+        assert (m ≠ n) as m_neq_n. 
+        { clear -m_notin_I0 n_in_I0. set_solver. }
+        assert (domm Im0 = {[m]}) as Domm_Im0.
+        { subst Im0. unfold domm, dom, flowint_dom.
+          unfold inf_map. simpl. apply leibniz_equiv. 
+          by rewrite dom_singleton. }
+        assert (domm Rm0 = {[m]}) as Domm_Rm0.
+        { subst Im0. unfold domm, dom, flowint_dom.
+          unfold inf_map. simpl. apply leibniz_equiv. 
+          by rewrite dom_singleton. }  
+        
+        iPoseProof (own_valid with "HI") as "%".
+        rename H into Valid_I0.
+        rewrite auth_auth_valid in Valid_I0 *; intros Valid_I0. 
+
+        iDestruct "HnS_si" as "(HnI & HnR & Domm_In0 & Domm_Rn0)".
+        iPoseProof (own_valid with "HnI") as "%".
+        rename H into Valid_In0. 
+        rewrite auth_frag_valid in Valid_In0 *; intros Valid_In0.
+        iPoseProof (own_valid with "HnR") as "%".
+        rename H into Valid_Rn0. 
+        rewrite auth_frag_valid in Valid_Rn0 *; intros Valid_Rn0.
+        iDestruct "Domm_In0" as %Domm_In0.
+        iDestruct "Domm_Rn0" as %Domm_Rn0.
+        
+        assert (✓ Im0) as Valid_Im0.
+        { unfold valid, cmra_valid, flowint_valid.
+          subst Im0. simpl. split.
+          solve_map_disjoint. 
+          intros _; try done. }
+        assert (✓ Rm0) as Valid_Rm0.
+        { unfold valid, cmra_valid, flowint_valid.
+          subst Rm0. simpl. split.
+          solve_map_disjoint. 
+          intros _; try done. }
+
+        iPoseProof ((auth_own_incl γ_I I0 In0) with "[$HI $HnI]") as "%".
+        rename H into Incl_In0. destruct Incl_In0 as [Iz Incl_In0].
+        iDestruct "Out_I" as %Out_I.
+        assert (out In0 m = 0%CCM ∧ out Iz m = 0%CCM) as [Out_In_m Out_Iz_m].
+        { unfold outflow_zero in Out_I.
+          rewrite Incl_In0 in Valid_I0*; intro H'.
+          rewrite Incl_In0 in m_notin_I0*; intro H''.
+          pose proof (intComp_unfold_out In0 Iz H' m H'') as Hout.
+          unfold out in Hout. unfold out.
+          rewrite <-Incl_In0 in Hout. rewrite Out_I in Hout. 
+          rewrite nzmap_lookup_empty in Hout. 
+          unfold ccmunit, ccm_unit in Hout. simpl in Hout.
+          unfold lift_unit in Hout. unfold ccmop, ccm_op in Hout.
+          simpl in Hout. unfold lift_op in Hout.
+          unfold ccmop, ccm_op in Hout. simpl in Hout.
+          rewrite nzmap_eq in Hout*; intros Hout.
+          unfold ccmunit, lift_unit. split; apply nzmap_eq;
+          intros k; rewrite nzmap_lookup_empty;
+          unfold ccmunit, ccm_unit; simpl;
+          unfold nat_unit; pose proof Hout k as Hout;
+          rewrite nzmap_lookup_empty in Hout;
+          unfold ccmunit, ccm_unit in Hout;
+          simpl in Hout; unfold nat_unit, nat_op in Hout;
+          rewrite nzmap_lookup_merge in Hout; clear-Hout; lia. }
+
+        assert (✓ (In0 ⋅ Im0)) as Valid_Inm0.
+        { apply intValid_composable. unfold intComposable.
+          repeat split; try done.
+          * simpl. solve_map_disjoint.
+          * rewrite Domm_In0 Domm_Im0.
+            clear -m_notin_I0 n_in_I0.
+            set_solver.
+          * unfold map_Forall. intros n' x Hinf.
+            subst Im0. unfold out. simpl.
+            rewrite nzmap_lookup_empty.
+            rewrite ccm_left_id. rewrite ccm_pinv_unit.
+            unfold inf. by rewrite Hinf.
+          * unfold map_Forall. intros n' x Hinf.
+            destruct (decide (n' = m)).
+            ** subst n'. rewrite Out_In_m.
+               rewrite ccm_left_id. rewrite ccm_pinv_unit.
+               unfold inf. by rewrite Hinf.
+            ** subst Im0. simpl in Hinf.
+               rewrite lookup_singleton_ne in Hinf; try done. }
+
+        assert (domm (In0 ⋅ Im0) = {[n; m]}) as Domm_Inm0.
+        { rewrite flowint_comp_fp; try done.
+          by rewrite Domm_In0 Domm_Im0. }
+        assert (domm I0 = domm In0 ∪ domm Iz) as Domm_Inz.
+        { rewrite Incl_In0. rewrite flowint_comp_fp. done.
+          by rewrite <-Incl_In0. }   
+        assert (n ∉ domm Iz) as n_notin_Iz.
+        { rewrite Incl_In0 in Valid_I0 *; intros Valid_In0'.
+          apply intComposable_valid in Valid_In0'.
+          unfold intComposable in Valid_In0'.
+          destruct Valid_In0' as [_ [_ [H' _]]].
+          rewrite Domm_In0 in H'. clear -H'; set_solver. }
+        assert (m ∉ domm Iz) as m_notin_Iz.
+        { clear -Domm_Inz m_notin_I0. set_solver. }
+          
+                
+        iMod (own_updateP (flowint_update_P (KT_multiset K) I0 In0 (In0 ⋅ Im0)) γ_I
+                   (● I0 ⋅ ◯ (In0)) with "[HI HnI]") as (Io) "H'".
+        { rewrite Incl_In0. apply flowint_update. 
+          split; last split.
+          - unfold contextualLeq.
+            repeat split; try done.
+            + rewrite flowint_comp_fp; try done.
+              clear; set_solver.
+            + intros n' H'.
+              assert (n' = n) as Hn.
+              { rewrite Domm_In0 in H'.
+                clear -H'; set_solver. }
+              subst n'.
+              pose proof (intComp_inf_1 In0 Im0 Valid_Inm0 n H') as H''.
+              rewrite H''. subst Im0; unfold out; simpl.
+              rewrite nzmap_lookup_empty.
+              by rewrite ccm_pinv_unit. 
+            + intros n' H'.
+              pose proof (intComp_unfold_out In0 Im0 Valid_Inm0 n' H') as H''.
+              rewrite H''. unfold out at 3, out_map. subst Im0.
+              simpl. rewrite nzmap_lookup_empty.
+              by rewrite ccm_right_id.
+          - rewrite Domm_Inm0. clear -n_notin_Iz m_notin_Iz.
+            set_solver.
+          - intros n' Hn'. rewrite Domm_Inm0 Domm_In0 in Hn'.
+            assert (n' = m) as H'. clear -Hn'. set_solver.
+            subst n'. by unfold out in Out_Iz_m. }              
+        { rewrite own_op. iFrame. }                        
+        iPoseProof ((flowint_update_result γ_I I0 In0 (In0 ⋅ Im0))
+                        with "H'") as (I0') "(% & % & (HI & HIn))".
+        rename H into ContLeq_I0. clear Io. 
+        destruct H1 as [Io [HI0 HI0']].
+        iEval (rewrite auth_frag_op) in "HIn".
+        iDestruct "HIn" as "(HIn & HIm)".
+        iPoseProof (own_valid with "HI") as "%".
+        rename H into Valid_I0'.
+        rewrite auth_auth_valid in Valid_I0' *; intros Valid_I0'. 
+
+        assert (domm I0' = domm I0 ∪ {[m]}) as Domm_I0'.
+        { rewrite Incl_In0 in HI0*; intros H'.
+          apply intComp_cancelable in H'. 
+          rewrite HI0'. repeat rewrite flowint_comp_fp.
+          rewrite Domm_Im0 H'. clear; set_solver.
+          rewrite Incl_In0 in Valid_I0 *; intros H''.
+          done. done. apply leibniz_equiv_iff in HI0'. 
+          by rewrite <-HI0'. by rewrite <-Incl_In0. }
+
+        assert (domm I0' ∖ {[m]} = domm I0) as Domm_I0_m.
+        { clear -Domm_I0' m_notin_I0. set_solver. }  
+
+        
+        iAssert (⌜r ∈ domm R0⌝)%I as "%". 
+        { iDestruct "domm_IR" as %H'. iPureIntro. by rewrite <-H'. }
+        rename H into r_in_R0.
+        iAssert (⌜m ∉ domm R0⌝)%I as "%".
+        { iDestruct "domm_IR" as %H'. iPureIntro. by rewrite <-H'. }
+        rename H into m_notin_R0.
+        iAssert (⌜n ∈ domm R0⌝)%I as "%".
+        { iDestruct "domm_IR" as %H'. iPureIntro. by rewrite <-H'. }
+        rename H into n_in_R0.        
+        
+        iPoseProof (own_valid with "HR") as "%".
+        rename H into Valid_R0.
+        rewrite auth_auth_valid in Valid_R0 *; intros Valid_R0. 
+        
+        iPoseProof ((auth_own_incl γ_R R0 Rn0) with "[$HR $HnR]") as "%".
+        rename H into Incl_Rn0. destruct Incl_Rn0 as [Rz Incl_Rn0].
+        iDestruct "Out_R" as %Out_R.
+        assert (out Rn0 m = 0%CCM ∧ out Rz m = 0%CCM) as [Out_Rn_m Out_Rz_m].
+        { unfold outflow_zero in Out_R.
+          rewrite Incl_Rn0 in Valid_R0*; intro H'.
+          rewrite Incl_Rn0 in m_notin_R0*; intro H''.
+          pose proof (intComp_unfold_out Rn0 Rz H' m H'') as Hout.
+          unfold out in Hout. unfold out.
+          rewrite <-Incl_Rn0 in Hout. rewrite Out_R in Hout. 
+          rewrite nzmap_lookup_empty in Hout. 
+          unfold ccmunit, ccm_unit in Hout. simpl in Hout.
+          unfold lift_unit in Hout. unfold ccmop, ccm_op in Hout.
+          simpl in Hout. unfold lift_op in Hout.
+          unfold ccmop, ccm_op in Hout. simpl in Hout.
+          rewrite nzmap_eq in Hout*; intros Hout.
+          unfold ccmunit, lift_unit. split; apply nzmap_eq;
+          intros k; rewrite nzmap_lookup_empty;
+          unfold ccmunit, ccm_unit; simpl;
+          unfold nat_unit; pose proof Hout k as Hout;
+          rewrite nzmap_lookup_empty in Hout;
+          unfold ccmunit, ccm_unit in Hout;
+          simpl in Hout; unfold nat_unit, nat_op in Hout;
+          rewrite nzmap_lookup_merge in Hout; clear-Hout; lia. }
+
+        assert (✓ (Rn0 ⋅ Rm0)) as Valid_Rnm0.
+        { apply intValid_composable. unfold intComposable.
+          repeat split; try done.
+          * simpl. solve_map_disjoint.
+          * rewrite Domm_Rn0 Domm_Rm0.
+            clear -m_notin_R0 n_in_R0.
+            set_solver.
+          * unfold map_Forall. intros n' x Hinf.
+            subst Rm0. unfold out. simpl.
+            rewrite nzmap_lookup_empty.
+            rewrite ccm_left_id. rewrite ccm_pinv_unit.
+            unfold inf. by rewrite Hinf.
+          * unfold map_Forall. intros n' x Hinf.
+            destruct (decide (n' = m)).
+            ** subst n'. rewrite Out_Rn_m.
+               rewrite ccm_left_id. rewrite ccm_pinv_unit.
+               unfold inf. by rewrite Hinf.
+            ** subst Rm0. simpl in Hinf.
+               rewrite lookup_singleton_ne in Hinf; try done. }
+
+        assert (domm (Rn0 ⋅ Rm0) = {[n; m]}) as Domm_Rnm0.
+        { rewrite flowint_comp_fp; try done.
+          by rewrite Domm_Rn0 Domm_Rm0. }
+        assert (domm R0 = domm Rn0 ∪ domm Rz) as Domm_Rnz.
+        { rewrite Incl_Rn0. rewrite flowint_comp_fp. done.
+          by rewrite <-Incl_Rn0. }   
+        assert (n ∉ domm Rz) as n_notin_Rz.
+        { rewrite Incl_Rn0 in Valid_R0 *; intros Valid_Rn0'.
+          apply intComposable_valid in Valid_Rn0'.
+          unfold intComposable in Valid_Rn0'.
+          destruct Valid_Rn0' as [_ [_ [H' _]]].
+          rewrite Domm_Rn0 in H'. clear -H'; set_solver. }
+        assert (m ∉ domm Rz) as m_notin_Rz.
+        { clear -Domm_Rnz m_notin_R0. set_solver. }               
+                
+        iMod (own_updateP (flowint_update_P (_) R0 Rn0 (Rn0 ⋅ Rm0)) γ_R
+                   (● R0 ⋅ ◯ (Rn0)) with "[HR HnR]") as (Ro) "H'".
+        { rewrite Incl_Rn0. apply flowint_update. 
+          split; last split.
+          - unfold contextualLeq.
+            repeat split; try done.
+            + rewrite flowint_comp_fp; try done.
+              clear; set_solver.
+            + intros n' H'.
+              assert (n' = n) as Hn.
+              { rewrite Domm_Rn0 in H'.
+                clear -H'; set_solver. }
+              subst n'.
+              pose proof (intComp_inf_1 Rn0 Rm0 Valid_Rnm0 n H') as H''.
+              rewrite H''. subst Rm0; unfold out; simpl.
+              rewrite nzmap_lookup_empty.
+              by rewrite ccm_pinv_unit. 
+            + intros n' H'.
+              pose proof (intComp_unfold_out Rn0 Rm0 Valid_Rnm0 n' H') as H''.
+              rewrite H''. unfold out at 3, out_map. subst Rm0.
+              simpl. rewrite nzmap_lookup_empty.
+              by rewrite ccm_right_id.
+          - rewrite Domm_Rnm0. clear -n_notin_Rz m_notin_Rz.
+            set_solver.
+          - intros n' Hn'. rewrite Domm_Rnm0 Domm_Rn0 in Hn'.
+            assert (n' = m) as H'. clear -Hn'. set_solver.
+            subst n'. by unfold out in Out_Rz_m. }              
+        { rewrite own_op. iFrame. }                        
+        iPoseProof ((flowint_update_result' γ_R R0 Rn0 (Rn0 ⋅ Rm0))
+                        with "H'") as (R0') "(% & % & (HR & HRn))".
+        rename H into ContLeq_R0. clear Ro. 
+        destruct H1 as [Ro [HR0 HR0']].
+        iEval (rewrite auth_frag_op) in "HRn".
+        iDestruct "HRn" as "(HRn & HRm)".
+        iPoseProof (own_valid with "HR") as "%".
+        rename H into Valid_R0'.
+        rewrite auth_auth_valid in Valid_R0' *; intros Valid_R0'. 
+
+        assert (domm R0' = domm R0 ∪ {[m]}) as Domm_R0'.
+        { rewrite Incl_Rn0 in HR0*; intros H'.
+          apply intComp_cancelable in H'. 
+          rewrite HR0'. repeat rewrite flowint_comp_fp.
+          rewrite Domm_Rm0 H'. clear; set_solver.
+          rewrite Incl_Rn0 in Valid_R0 *; intros H''.
+          done. done. apply leibniz_equiv_iff in HR0'. 
+          by rewrite <-HR0'. by rewrite <-Incl_Rn0. }
+        assert (domm R0' ∖ {[m]} = domm R0) as Domm_R0_m.
+        { clear -Domm_R0' m_notin_R0. set_solver. }
+        iDestruct "Inf_R" as %Inf_R.  
+        iAssert (⌜inflow_R R0' r⌝)%I as "Inf_R'".
+        { iPureIntro. unfold inflow_R. intros n' k.
+          destruct (n' =? r) eqn: Hn'.
+          + pose proof Inf_R n' k as Inf_R.
+            rewrite Hn' in Inf_R.
+            rewrite Nat.eqb_eq in Hn'*; intros Hn'.
+            subst n'. unfold contextualLeq in ContLeq_R0.
+            destruct ContLeq_R0 as [_ [_ [_ [H' _]]]].
+            pose proof H' r r_in_R0 as H'.
+            unfold in_inset. unfold in_inset in Inf_R.
+            by rewrite <-H'. 
+          + pose proof Inf_R n' k as Inf_R.
+            rewrite Hn' in Inf_R.
+            rewrite Nat.eqb_neq in Hn'*; intros Hn'.
+            unfold contextualLeq in ContLeq_R0.
+            destruct ContLeq_R0 as [_ [_ [_ [H' H'']]]].
+            destruct (decide (n' ∈ domm R0)).
+            * pose proof H' n' e as H'.
+              unfold in_inset. unfold in_inset in Inf_R.
+              by rewrite <-H'.
+            * destruct (decide (n' = m)).
+              ** subst n'.
+                 pose proof (intComp_inf_2 R0 Rm0) as Hinf.
+                 rewrite cmra_comm in HR0' *; intros HR0'.
+                 rewrite cmra_assoc in HR0' *; intros HR0'.
+                 rewrite cmra_comm in HR0 *; intros HR0.
+                 rewrite <-HR0 in HR0'.
+                 rewrite HR0' in Valid_R0'.
+                 assert (m ∈ domm Rm0) as m_in_Rm0.
+                 { rewrite Domm_Rm0. clear; set_solver. }
+                 pose proof Hinf Valid_R0' m m_in_Rm0 as Hinf.
+                 apply leibniz_equiv_iff in HR0'. 
+                 rewrite <-HR0' in Hinf.
+                 unfold in_inset. rewrite Hinf.
+                 unfold outflow_zero_R in Out_R.
+                 unfold out. rewrite Out_R.
+                 rewrite nzmap_lookup_empty.
+                 subst Rm0. unfold inf. simpl.
+                 rewrite lookup_singleton.
+                 simpl. rewrite ccm_pinv_unit.
+                 clear. unfold dom_ms, dom, nzmap_dom.
+                 set_solver.
+              ** assert (n' ∉ domm R0') as Hdom.
+                 { rewrite Domm_R0'.
+                   clear -n0 n1. set_solver. }
+                 unfold domm, dom, flowint_dom in Hdom.
+                 destruct R0' as [ [Rinf Rout] | ]; last by contradiction.
+                 simpl in Hdom. rewrite not_elem_of_dom in Hdom *; intros Hdom.
+                 unfold in_inset. unfold inf, inf_map.
+                 simpl. rewrite Hdom. simpl.
+                 unfold ccmunit, ccm_unit, lift_unit.
+                 unfold dom_ms, dom, flowint_dom, nzmap_dom.
+                 unfold nzmap_unit. simpl. clear; set_solver. }
+        iMod (own_update γ_f (● domm I0) (● (domm I0 ∪ {[m]}) ⋅ ◯ ({[m]}))
+                         with "[Hf]") as "(Hf & H')"; try done.
+        { apply (auth_update_alloc (domm I0) (domm I0 ∪ {[m]}) ({[m]})).
+          apply local_update_discrete.
+          intros mz _ Hmz. split; try done.
+          rewrite gset_opM in Hmz. rewrite gset_opM.
+          rewrite Hmz. clear. set_solver. }
+        iEval (rewrite <-Domm_I0') in "Hf".
+        iAssert (inFP γ_f m) with "H'" as "#FP_m".
+        iDestruct "H'" as "HnS_FPm".
+        
+        iMod (own_alloc (to_frac_agree (1) (esm0))) 
+              as (γ_em)"Hesm_f". { try done. }
+        iEval (rewrite <-Qp_half_half) in "Hesm_f".      
+        iEval (rewrite (frac_agree_op (1/2) (1/2) _)) in "Hesm_f". 
+        iDestruct "Hesm_f" as "(HnS_esm & HnP_esm)".        
+
+        iMod (own_alloc (to_frac_agree (1) (Cm0))) 
+              as (γ_cm)"Hcm_f". { try done. }
+        iEval (rewrite <-Qp_half_half) in "Hcm_f".      
+        iEval (rewrite (frac_agree_op (1/2) (1/2) _)) in "Hcm_f". 
+        iDestruct "Hcm_f" as "(HnS_cm & HnP_cm)".        
+
+        iMod (own_alloc (to_frac_agree (1) (Bm0))) 
+              as (γ_bm)"Hbm_f". { try done. }
+        iEval (rewrite <-Qp_half_half) in "Hbm_f".      
+        iEval (rewrite (frac_agree_op (1/2) (1/2) _)) in "Hbm_f". 
+        iDestruct "Hbm_f" as "(HnS_bm & HnP_bm)".        
+
+        iMod (own_alloc (to_frac_agree (1) (Qm0))) 
+              as (γ_qm)"Hqm_f". { try done. }
+        iEval (rewrite <-Qp_half_half) in "Hqm_f".      
+        iEval (rewrite (frac_agree_op (1/2) (1/2) _)) in "Hqm_f". 
+        iDestruct "Hqm_f" as "(HnS_qm & HnP_qm)".
+        
+        iAssert (frac_ghost_state γ_em γ_cm γ_bm γ_qm esm0 Cm0 Bm0 Qm0
+                ∗ frac_ghost_state γ_em γ_cm γ_bm γ_qm esm0 Cm0 Bm0 Qm0)%I
+                with "[HnS_esm HnP_esm HnS_cm HnP_cm HnS_bm HnP_bm HnS_qm HnP_qm]"
+                as "(HnS_fracm & HnP_fracm)".
+        { iFrame. }               
+
+        iMod (own_alloc_set KS with "[]") as "HnS_starm"; first done.
+        iDestruct "HnS_starm" as (γ_cirm)"HnS_starm".
+        
+        iDestruct "domm_IR" as "#domm_IR".
+        iDestruct "domm_Iγ" as "#domm_Iγ".
+        iMod ((ghost_heap_update γ_gh hγ0 m γ_em γ_cm γ_bm γ_qm γ_cirm) 
+                    with "[] [$Hγ]") as "(Hγ & #HnS_ghm)".
+        { iDestruct "domm_Iγ" as %H'. iPureIntro.
+          rewrite <-H'. apply m_notin_I0. }            
+
+        assert (set_of_map Cm0 = ∅) as Set_of_Cm0.
+        { unfold set_of_map. subst Cm0.
+          by rewrite map_fold_empty. }
+        iMod (own_update γ_s (● H0) (● H0 ⋅ ◯ (set_of_map Cm0))
+                 with "[$HH]") as "HH".
+        { apply (auth_update_alloc _ (H0) (set_of_map Cm0)).
+          rewrite Set_of_Cm0.
+          apply local_update_discrete. intros mz Valid_H1 H1_eq.
+          split; try done. }
+        iDestruct "HH" as "(HH & HnP_Cm)".
+        
+        iAssert (closed γ_f esm0) as "HnS_clm".
+        { iIntros (n')"%". rename H into H'.
+          exfalso. rewrite Hesm in H'.
+          rewrite /(∅ !!! n') in H'.
+          unfold finmap_lookup_total in H'.
+          rewrite lookup_empty in H'.
+          simpl in H'. clear -H'; done. }
+
+        set (Sr := esn' !!! m ∩ inset K Rn0 n).
+        set (Sr_map := map_restriction Sr ∅).
+        set (Sr_mset := map_subset Sr ∅).
+        set (Sb := Sr ∖ dom (gset K) Cn).
+        set (Sb_map := map_restriction Sb ∅). 
+        set (Qn0' := gmap_insert_map Qn Sr_map).
+        set (Bn0' := gmap_insert_map Bn Sb_map).
+        set (In0' := outflow_insert_set_KT In0 m Sr_mset).
+        set (Im0' := inflow_insert_set_KT Im0 m Sr_mset). 
+        set (Rn0' := outflow_insert_set_K Rn0 m Sr).
+        set (Rm0' := inflow_insert_set_K Rm0 m Sr).
+
+        iMod ((frac_update γ_en γ_cn γ_bn γ_qn esn Cn Bn Qn esn' Cn Bn0' Qn0') 
+             with "[$HnP_frac $HnS_frac]") as "(HnP_frac & HnS_frac)".
+
+        iAssert (closed γ_f esn')%I with "[HnS_cl]" as "HnS_cl".
+        { unfold closed. iIntros (n')"%". rename H into Hn'.
+          destruct (decide (n' = m)).
+          + subst n'; try done.
+          + rewrite Hesn' in Hn'.
+            rewrite lookup_total_insert_ne in Hn'; try done.
+            iApply "HnS_cl". by iPureIntro. }
+
+        iAssert (own γ_R (◯ Rn0') ∗ own γ_R (◯ Rm0'))%I 
+                with "[HRn HRm]" as "(HRn & HRm)".
+        { iCombine "HRn HRm" as "HRnm".
+          assert (Rn0' = outflow_insert_set_K Rn0 m Sr) 
+                  as HRn0'. done.
+          assert (Rm0' = inflow_insert_set_K Rm0 m Sr)
+                  as HRm0'. done.         
+          pose proof (flowint_insert_set_eq_K Rn0 Rn0' Rm0 Rm0' 
+                  m Sr HRn0' HRm0') as HRnm0'.
+          iEval (rewrite HRnm0') in "HRnm".
+          iEval (rewrite auth_frag_op) in "HRnm".
+          iDestruct "HRnm" as "(?&?)". iFrame. }
+
+        iAssert (own γ_I (◯ In0') ∗ own γ_I (◯ Im0'))%I 
+                with "[HIn HIm]" as "(HIn & HIm)".
+        { iCombine "HIn HIm" as "HInm".
+          assert (In0' = outflow_insert_set_K In0 m Sr_mset) 
+                  as HIn0'. done.
+          assert (Im0' = inflow_insert_set_K Im0 m Sr_mset)
+                  as HIm0'. done.         
+          pose proof (flowint_insert_set_eq_KT In0 In0' Im0 Im0' 
+                  m Sr_mset HIn0' HIm0') as HInm0'.
+          iEval (rewrite HInm0') in "HInm".
+          iEval (rewrite auth_frag_op) in "HInm".
+          iDestruct "HInm" as "(?&?)". iFrame. }
+
+        assert (domm Rm0' = {[m]}) as Domm_Rm0'.
+        { admit. }         
+
+        assert (domm Im0' = {[m]}) as Domm_Im0'.
+        { admit. }         
+
+        assert (esn !!! m = ∅) as Esn_empty.
+        { admit. }
+
+        iPoseProof ((node_edgeset_disjoint r n) with "[$node_n]") as "%".
+        rename H into Disj_esn'.                        
+
+
+        iAssert (⌜φ0 esn Qn⌝)%I as "%".
+        { by iDestruct "Hφ" as "(%&_)". }
+        rename H into Hφ0.
+
+        assert (∀ k, k ∈ Sr → Qn0' !! k = Some 0) as Lookup_Qn0'.
+        { admit. }
+
+        assert (∀ k, k ∉ Sr → Qn0' !! k = Qn !! k) as Lookup_Qn0'_ne.
+        { admit. }
+
+        assert (∀ k, k ∈ Sb → Bn0' !! k = Some 0) as Lookup_Bn0'.
+        { admit. }
+
+        assert (∀ k, k ∉ Sb → Bn0' !! k = Bn !! k) as Lookup_Bn0'_ne.
+        { admit. }
+        
+        assert (∀ k t, (k, t) ∈ Sr_mset ↔ k ∈ Sr ∧ t = 0) as HSr_mset.
+        { admit. }
+
+        assert (∀ k, k ∈ Sr → (∀ n', k ∉ esn !!! n')) as Esn_not.
+        { admit. } 
+
+        assert (∀ k, k ∈ Sb → Bn !!! k = 0) as HSb.
+        { admit. }
+
+        iAssert (⌜∀ k, Bn !!! k ≤ Bn0' !!! k⌝)%I as "%".
+        { admit. }
+        rename H into Bn_le_Bn0'.
+
+        iAssert (|==> [∗ set] k ∈ KS, own (γ_cirn !!! k)
+                                (● {| max_nat_car := Bn0' !!! k |}))%I
+                      with "[HnS_star]" as ">HnS_star".
+        { iInduction KS as [| s S'] "IHs" using set_ind_L.
+          - admit.
+          - admit. }
+
+
+        iDestruct "HnS_oc" as "(%&%&%)".
+        rename H into OC1. rename H1 into OC2. rename H2 into OC3.
+
+        iAssert (outflow_constraints n In0' Rn0' esn' Qn0')%I as "HnS_oc".
+        { iPureIntro. split; last split; try done.
+          - intros n' k t. destruct (decide (n' = m)).
+            + subst n'. assert (outset_KT In0' m = Sr_mset) as Hout.
+              { admit. } rewrite Hout. split.
+              * intros H'. apply HSr_mset in H'. 
+                destruct H' as [H1' H2'].
+                split. subst Sr. clear -H1'. set_solver.
+                rewrite (Lookup_Qn0' k H1').
+                by rewrite H2'.
+              * intros [Hkt1 Hkt2].
+                destruct (decide (k ∈ Sr)).
+                ** rewrite (Lookup_Qn0' k e) in Hkt2.
+                   inversion Hkt2. rewrite HSr_mset.
+                   split; try done. 
+                ** assert (∀ n', k ∉ esn !!! n') as Hnot.
+                   { intros n'. destruct (decide (n' = m)).
+                     subst n'. rewrite Esn_empty. clear; set_solver.
+                     destruct (decide (k ∈ esn !!! n')); try done.
+                     assert (k ∈ esn' !!! n') as H'. rewrite Hesn'. 
+                     rewrite lookup_total_insert_ne; try done.
+                     pose proof Disj_esn' n' m n1 as Disj_esn'.
+                     clear -Disj_esn' Hkt1 H'. set_solver. }
+                   rewrite (Lookup_Qn0'_ne k n0) in Hkt2.   
+                   pose proof Hφ0 k Hnot as H'. rewrite H' in Hkt2.
+                   done.
+            + rewrite Hesn'. rewrite lookup_total_insert_ne; try done.
+              assert (outset_KT In0' n' = outset_KT In0 n') as Hout.
+              { admit. } rewrite Hout. split.
+              * destruct (decide (k ∈ Sr)).
+                ** intros H'. apply OC1 in H'.
+                   admit.
+                ** rewrite (Lookup_Qn0'_ne k n1). apply OC1.   
+              * intros [Hkt1 Hkt2]. destruct (decide (k ∈ Sr)).
+                ** admit.
+                **rewrite (Lookup_Qn0'_ne k n1) in Hkt2.
+                  apply OC1; try done.   
+          - intros n' k. assert (inset K Rn0' n = inset K Rn0 n) as Hin.
+            { try done. } rewrite Hin. destruct (decide (n' = m)).
+            + subst n'. assert (outset K Rn0' m = Sr) as Hout.
+              { admit. } rewrite Hout. 
+              subst Sr.  rewrite elem_of_intersection.
+              split; try done.
+            + assert (outset K Rn0' n' = outset K Rn0 n') as Hout.
+              { admit. } rewrite Hout. rewrite Hesn'. 
+              rewrite lookup_total_insert_ne; try done.
+          - intros n' kt. destruct (decide (n' = m)).
+            + subst n'. subst In0'. admit.
+            + subst In0'. unfold outflow_insert_set_KT.
+              unfold out at 1, out_map at 1; simpl.
+              rewrite nzmap_lookup_total_insert_ne; try done.
+              pose proof OC3 n' kt as H'. by unfold out in H'.  }
+       
+        iAssert (outflow_constraints m Im0' Rm0' esm0 Qm0)%I as "HnS_ocm".
+        { iPureIntro. split; last split.
+          - split.
+            + unfold outset_KT, KT_flows.dom_ms. 
+              rewrite nzmap_elem_of_dom_total. unfold out, out_map. 
+              subst Im0. simpl. rewrite nzmap_lookup_empty. 
+              unfold ccmunit, ccm_unit. simpl.
+              unfold lift_unit.
+              rewrite nzmap_lookup_empty.
+              unfold ccmunit, ccm_unit. simpl. done.
+            + subst esm0. rewrite /(∅ !!! n'). 
+              unfold finmap_lookup_total. rewrite lookup_empty.
+              simpl. clear; set_solver.
+          - unfold outflow_constraint_R. 
+            intros n' k. unfold outset.
+            assert (out Rm0' n' = out Rm0 n') as Hout.
+            { admit. } rewrite Hout. split.
+            + unfold in_outset, dom_ms. 
+              rewrite nzmap_elem_of_dom_total. unfold out, out_map. 
+              subst Rm0. simpl. rewrite nzmap_lookup_empty. 
+              unfold ccmunit, ccm_unit. simpl.
+              unfold lift_unit.
+              rewrite nzmap_lookup_empty.
+              unfold ccmunit, ccm_unit. simpl. done.
+            + subst esm0. rewrite /(∅ !!! n'). 
+              unfold finmap_lookup_total. rewrite lookup_empty.
+              simpl. clear; set_solver.
+          - intros n' kt. unfold out, out_map; subst Im0; simpl.
+            rewrite nzmap_lookup_empty. unfold ccmunit, ccm_unit.
+            simpl. unfold lift_unit. rewrite nzmap_lookup_empty.
+            unfold ccmunit, ccm_unit; simpl. unfold nat_unit. lia. }
+
+        iAssert (⌜φ0 esn' Qn0'⌝ ∗ ⌜φ1 Bn0' Cn Qn0'⌝ ∗ ⌜φ2 n Bn0' In0'⌝ 
+           ∗ ⌜φ3 n Bn0' Rn0'⌝ ∗ ⌜φ4 n Rn0'⌝ ∗ ⌜φ5 Bn0' Qn0'⌝ 
+           ∗ ⌜φ6 Bn0' T0'⌝ ∗ ⌜φ7 n esn' Rn0' Qn0'⌝)%I 
+                with "[Hφ]" as "Hφ".
+        { iDestruct "Hφ" as "(%&%&%&%&%&%&%&%)".         
+          clear H. rename H1 into Hφ1. 
+          rename H2 into Hφ2. rename H3 into Hφ3.
+          rename H4 into Hφ4. rename H5 into Hφ5.
+          rename H6 into Hφ6. rename H7 into Hφ7.
+          iPureIntro. split; last split; last split; 
+          last split; last split; last split; last split.
+          - intros k Hnot. destruct (decide (k ∈ Sr)). 
+            + admit. 
+            + rewrite (Lookup_Qn0'_ne k n0). apply Hφ0. 
+              intros n'. destruct (decide (n' = m)).
+              * subst n'. rewrite Esn_empty.
+                clear; set_solver.
+              * pose proof Hnot n' as Hnot.
+                rewrite Hesn' in Hnot.
+                rewrite lookup_total_insert_ne in Hnot; try done.
+          - intros k t. destruct (decide (k ∈ Sr)).
+            + split.
+              * assert (k ∉ Sb) as Hk.
+                { admit. }
+                rewrite (Lookup_Bn0'_ne k Hk).
+                apply Hφ1.
+              * assert (k ∈ Sb) as Hk.
+                { admit. }
+                rewrite (Lookup_Bn0' k Hk).
+                rewrite (Lookup_Qn0' k e).
+                done.
+            + assert (k ∉ Sb) as Hk.
+              { admit. }
+              rewrite (Lookup_Bn0'_ne k Hk).
+              rewrite (Lookup_Qn0'_ne k n0).
+              apply Hφ1.
+          - intros k t. assert (inset_KT In0' n = inset_KT In0 n) as Hin. 
+            { admit. } rewrite Hin. destruct (decide (k ∈ Sb)). 
+            + intros H'. apply Hφ2 in H'. rewrite lookup_total_alt.
+              rewrite (Lookup_Bn0' k e). simpl.
+              by rewrite (HSb k e) in H'.
+            + rewrite lookup_total_alt. rewrite (Lookup_Bn0'_ne k n0).
+              rewrite <-lookup_total_alt. apply Hφ2.
+          - intros k. assert (inset K Rn0' n = inset K Rn0 n) as Hin.
+            { admit. } rewrite Hin.
+            destruct (decide (k ∈ Sb)).
+            + right. subst Sb. subst Sr. clear -e. set_solver.
+            + by rewrite (Lookup_Bn0'_ne k n0).
+          - try done.
+          - intros k. destruct (decide (k ∈ Sb)).
+            + destruct (decide (k ∈ Sr)).
+              * rewrite !lookup_total_alt. 
+                rewrite (Lookup_Bn0' k e).
+                rewrite (Lookup_Qn0' k e0).
+                by simpl.
+              * subst Sb Sr; clear -e n0; set_solver.
+            + destruct (decide (k ∈ Sr)).
+              * rewrite lookup_total_alt.
+                rewrite (Lookup_Qn0' k e).
+                simpl. lia.
+              * rewrite !lookup_total_alt. 
+                rewrite (Lookup_Bn0'_ne k n0).
+                rewrite (Lookup_Qn0'_ne k n1).
+                rewrite <-!lookup_total_alt.
+                by apply Hφ5.
+          - intros k. admit.
+          - intros k. intros [H' H''].
+            destruct H' as [n' H'].
+            destruct (decide (n' = m)).
+            + subst n'. admit.
+            + assert (inset K Rn0' n = inset K Rn0 n) as Hin.
+              { admit. } rewrite Hesn' in H'.
+              rewrite lookup_total_insert_ne in H'; try done.
+              destruct (decide (k ∈ Sr)).
+              * pose proof Lookup_Qn0' k e as H'''.
+                admit.
+              * rewrite elem_of_dom. rewrite (Lookup_Qn0'_ne k n1).
+                rewrite <-elem_of_dom. apply Hφ7.
+                split; try done. by exists n'. }
+      
+        iAssert (⌜φ0 esm0 Qm0⌝ ∗ ⌜φ1 Bm0 Cm0 Qm0⌝ ∗ ⌜φ2 m Bm0 Im0'⌝ 
+              ∗ ⌜φ3 m Bm0 Rm0'⌝ ∗ ⌜φ4 m Rm0'⌝ ∗ ⌜φ5 Bm0 Qm0⌝  
+              ∗ ⌜φ6 Bm0 T0'⌝ ∗ ⌜φ7 m esm0 Rm0' Qm0⌝)%I
+                 as "Hφm".
+        { iPureIntro. subst esm0 Cm0 Bm0 Qm0.
+          repeat split; try done.
+          - unfold φ2.
+            assert (inset_KT Im0' m = Sr_mset) as Hin.
+            { admit. } rewrite Hin. intros k t Hkt.
+            apply HSr_mset in Hkt.
+            destruct Hkt as [_ H'].
+            rewrite lookup_total_alt; rewrite lookup_empty; by simpl.
+          - unfold φ3. intros k; left.
+            rewrite /(∅ !!! k). unfold finmap_lookup_total.
+            rewrite lookup_empty. by simpl.
+          - unfold φ4. intros k.
+            subst Rm0; unfold inf, inf_map; simpl.
+            rewrite lookup_insert. simpl.
+            unfold inf, inf_map; simpl.
+            rewrite lookup_insert. simpl.
+            admit.
+          - intros k. rewrite /(∅ !!! k).
+            unfold finmap_lookup_total.
+            rewrite lookup_empty. by simpl.  
+          - unfold φ6. intros k. rewrite /(∅ !!! k). 
+            unfold finmap_lookup_total. rewrite lookup_empty.
+            simpl. lia.
+          - intros k [Hkt1 Hkt2].
+            destruct Hkt1 as [n' H'].
+            clear -H'. set_solver.   }
+
+        iAssert (⌜outflow_zero I0'⌝)%I as "Out_I'".
+        { iPureIntro. unfold outflow_zero.
+          apply nzmap_eq. intros n'.
+          destruct (decide (n' ∈ domm I0')).
+          + pose proof intValid_in_dom_not_out I0' n' Valid_I0' e as H'.
+            unfold out in H'. rewrite H'.
+            by rewrite nzmap_lookup_empty.
+          + destruct ContLeq_I0 as [_ [_ [_ [H' H'']]]].
+            pose proof H'' n' n0 as H''.
+            unfold out in H''. rewrite <-H''.
+            apply leibniz_equiv in Out_I.
+            rewrite nzmap_eq in Out_I *; intros Out_I.
+            pose proof Out_I n' as Out_I.
+            by rewrite Out_I. }  
+
+        iAssert (⌜outflow_zero_R R0'⌝)%I as "Out_R'".
+        { iPureIntro. unfold outflow_zero.
+          apply nzmap_eq. intros n'.
+          destruct (decide (n' ∈ domm R0')).
+          + pose proof intValid_in_dom_not_out R0' n' Valid_R0' e as H'.
+            unfold out in H'. rewrite H'.
+            by rewrite nzmap_lookup_empty.
+          + destruct ContLeq_R0 as [_ [_ [_ [H' H'']]]].
+            pose proof H'' n' n0 as H''.
+            unfold out in H''. rewrite <-H''.
+            apply leibniz_equiv in Out_R.
+            rewrite nzmap_eq in Out_R *; intros Out_R.
+            pose proof Out_R n' as Out_R.
+            by rewrite Out_R. }  
+
+        iAssert (⌜bn = true⌝)%I as "%".
+        { destruct bn; try done.
+          iDestruct "Hlif_n" as 
+              (γ_er' γ_cr' γ_br' γ_qr' γ_cirr' es' T'')"(node' & _)".
+          iPoseProof ((node_sep_star r n) with "[$]") as "%".
+          contradiction. } subst bn.
+
+
+        iModIntro. iSplitR "AU node_n HnP_gh HnP_frac HnP_C HnP_t".
+        { iNext. iExists T0', H0,
+               (<[m:=ghost_loc γ_em γ_cm γ_bm γ_qm γ_cirm]> hγ0), I0', R0'.
+          iSplitL "MCS_auth Hist Ht FP_r Max_ts HI HR Hf Hγ HH Out_I' Out_R'".
+          { iFrame. iFrame "Inf_R' Out_I' Out_R'". 
+            iDestruct "domm_IR" as %H'.
+            iDestruct "domm_Iγ" as %H''.
+            iPureIntro. split.
+            rewrite Domm_I0' Domm_R0'. by rewrite H'.
+            apply leibniz_equiv. rewrite dom_insert.
+            rewrite Domm_I0' H''. clear; set_solver. }
+          rewrite (big_sepS_delete _ (domm I0') m); 
+              last first. { rewrite Domm_I0'. clear; set_solver. }
+          iSplitR "Hl_n Hlif_n HnS_gh HnS_frac
+                      HnS_FP HnS_cl HnS_oc HnS_H HnS_star Hφ Hstar' HIn HRn".
+          { iExists false, Cm0, Bm0, Qm0. iFrame "Hl_m".
+            iSplitL "node_m HnP_fracm HnP_Cm". 
+            iExists γ_em, γ_cm, γ_bm, γ_qm, γ_cirm, esm0, T.
+            iFrame "∗#".
+            rewrite <-(PeanoNat.Nat.eqb_neq m r) in m_neq_r.
+            by rewrite m_neq_r.
+            iExists γ_em, γ_cm, γ_bm, γ_qm, γ_cirm, esm0, Im0', Rm0'.
+            iFrame "∗#". repeat iSplitR; try by iPureIntro.
+            rewrite <-(PeanoNat.Nat.eqb_neq m r) in m_neq_r.
+            by rewrite m_neq_r.
+            iApply (big_sepS_mono 
+                    (λ y, own (γ_cirm !!! y) (● {| max_nat_car := 0 |}) )%I
+                    (λ y, own (γ_cirm !!! y) (● {| max_nat_car := Bm0 !!! y |}))%I
+                    KS); try done. }
+            rewrite Domm_I0_m.
+            rewrite (big_sepS_delete _ (domm I0) n); 
+              last apply n_in_I0.
+            iFrame "Hstar'". iExists true, Cn, Bn0', Qn0'.
+            iFrame. iExists γ_en, γ_cn, γ_bn, γ_qn, γ_cirn, esn', In0', Rn0'.
+            iFrame "∗#". destruct (n =? r). 
+            - iDestruct "HnS_H" as "(%&%)". 
+              iPureIntro. repeat split; try done.
+              admit. }
+
+        iModIntro.
+        iClear "Inf_R' domm_IR domm_Iγ HnS_clm HnS_ocm Hφm Out_I' Out_R' HnS_oc".
+        clear In0' Im0' Domm_Im0' OC1 OC2 OC3 Hcm Hesm m_notin_I0 
+        n_in_I0 In0 Qm0 Bm0 Im0 r_in_I0 Domm_Im0 Domm_Rm0 Valid_I0 Valid_In0
+        Valid_Rn0 Domm_In0 Domm_Rn0 Valid_Im0 Valid_Rm0 Iz Incl_In0
+        Out_I Out_In_m Out_Iz_m Valid_Inm0 Domm_Inm0 Domm_Inz
+        n_notin_Iz m_notin_Iz I0' ContLeq_I0 Io HI0 HI0' Valid_I0'
+        Domm_I0' Domm_I0_m r_in_R0 m_notin_R0 n_in_R0 Valid_R0
+        Rz Incl_Rn0 Out_R Out_Rn_m Out_Rz_m Valid_Rnm0 Domm_Rnm0
+        Domm_Rnz n_notin_Rz m_notin_Rz R0' ContLeq_R0 R0 HR0
+        HR0' Valid_R0' Domm_R0' Domm_R0_m Inf_R Set_of_Cm0 Hφ0.
+        clear Disj_esn esm0 Cm0 T0' hγ0 I0 Ro
+        Rn0' Rm0' Domm_Rm0' Domm_Rm0' Esn_empty.
+        
+        awp_apply lockNode_spec_high without "HnP_t"; try done.
+        iAaccIntro with ""; try eauto with iFrame.
+        iIntros (Cm Bm Qm)"HnP_m". iModIntro.
+        iIntros "HnP_t". wp_pures.
+        iDestruct "HnP_m" as (γ_em' γ_cm' γ_bm' γ_qm' γ_cirm' esm Tm)"(node_m   
+                            & HnP_ghm & HnP_fracm & HnP_Cm & HnP_tm)".
+        iPoseProof (ghost_heap_sync with "[$HnP_ghm] [$HnS_ghm]") 
+                                  as "(% & % & % & % & %)".
+        subst γ_em'. subst γ_cm'. subst γ_bm'. subst γ_qm'. subst γ_cirm'.
+        wp_apply (mergeContents_spec with "[$node_n $node_m]"); try done.
+        iIntros (Cn' Cm') "(node_n & node_m & Subset_Cn & Subset_Cm 
+                                         & Subset_disj & MergeEq)".  
+        iDestruct "Subset_Cn" as %Subset_Cn.
+        iDestruct "Subset_Cm" as %Subset_Cm.
+        iDestruct "Subset_disj" as %Subset_disj.
+        iDestruct "MergeEq" as %MergeEq. wp_pures.
+        iApply fupd_wp. iInv "HInv" as ">H".
+        iDestruct "H" as (T' H hγ I R) "(Hglob & Hstar)".
+        iAssert (⌜n ∈ domm I⌝)%I as "%". 
+        { iDestruct "Hglob" as "(MCS_auth & HH & Hist & Ht & HI & Out_I & HR 
+            & Out_R & Inf_R & Hf & Hγ & FP_r & Max_ts & domm_IR & domm_Iγ)".
+          by iPoseProof (inFP_domm _ _ _ with "[$FP_n] [$Hf]") as "H'". }
+        rename H1 into n_in_I.  
+        rewrite (big_sepS_delete _ (domm I) n); last by eauto.
+        iDestruct "Hstar" as "(H_n & Hstar')".
+        iDestruct "H_n" as (bn Cn'' Bn'' Qn'')"(Hl_n & Hlif_n & HnS_n)".
+        iDestruct "HnS_n" as (γ_en' γ_cn' γ_bn' γ_qn' γ_cirn' es' In Rn) 
+                      "(HnS_gh & HnS_frac & HnS_si & HnS_FP 
+                                & HnS_cl & HnS_oc & HnS_H & HnS_star & Hφ)".
+        iPoseProof (ghost_heap_sync with "[$HnP_gh] [$HnS_gh]") 
+                                  as "(% & % & % & % & %)".
+        subst γ_en'. subst γ_cn'. subst γ_bn'. subst γ_qn'. subst γ_cirn'.
+        iPoseProof (frac_eq with "[$HnP_frac] [$HnS_frac]") as "%".
+        destruct H1 as [Hes [Hc [Hb Hq]]]. 
+        subst es'. subst Cn''. subst Bn''. subst Qn''.
+        iAssert (⌜m ∈ domm I⌝)%I as "%". 
+        { iDestruct "Hglob" as "(MCS_auth & HH & Hist & Ht & HI & Out_I & HR 
+            & Out_R & Inf_R & Hf & Hγ & FP_r & Max_ts & domm_IR & domm_Iγ)".
+          by iPoseProof (inFP_domm _ _ _ with "[$FP_m] [$Hf]") as "H'". }
+        rename H1 into m_in_I.
+        rewrite (big_sepS_delete _ (domm I ∖ {[n]}) m); last by set_solver.
+        iDestruct "Hstar'" as "(H_m & Hstar')".
+        iDestruct "H_m" as (bm Cm'' Bm'' Qm'')"(Hl_m & Hlif_m & HnS_m)".
+        iClear "HnS_ghm".
+        iDestruct "HnS_m" as (γ_em' γ_cm' γ_bm' γ_qm' γ_cirm' es' Im Rm) 
+                      "(HnS_ghm & HnS_fracm & HnS_sim & HnS_FPm 
+                                & HnS_clm & HnS_ocm & HnS_Hm & HnS_starm & Hφm)".
+        iPoseProof (ghost_heap_sync with "[$HnP_ghm] [$HnS_ghm]") 
+                                  as "(% & % & % & % & %)".
+        subst γ_em'. subst γ_cm'. subst γ_bm'. subst γ_qm'. subst γ_cirm'.
+        iPoseProof (frac_eq with "[$HnP_fracm] [$HnS_fracm]") as "%".
+        destruct H1 as [Hes [Hc [Hb Hq]]]. 
+        subst es'. subst Cm''. subst Bm''. subst Qm''.
+
+        iAssert (⌜bn = true⌝)%I as "%".
+        { destruct bn; try done.
+          iDestruct "Hlif_n" as 
+              (γ_er' γ_cr' γ_br' γ_qr' γ_cirr' es' T'')"(node' & _)".
+          iPoseProof ((node_sep_star r n) with "[$]") as "%".
+          contradiction. } subst bn.
+                
+        iAssert (⌜bm = true⌝)%I as "%".
+        { destruct bm; try done.
+          iDestruct "Hlif_m" as 
+              (γ_er' γ_cr' γ_br' γ_qr' γ_cirr' es' T'')"(node' & _)".
+          iPoseProof ((node_sep_star r m) with "[$]") as "%".
+          contradiction. } subst bm.
+        
+        set (S := dom (gset K) Cn ∖ dom (gset K) Cn').
+        set (S_map := map_restriction S Cn).
+        set (Qn_old := map_subset S Qn0').
+        set (Qn_new := map_subset S Cn).
+        set (Qn' := gmap_insert_map Qn0' S_map).
+        set (Bm' := gmap_insert_map Bm S_map).
+        set (In_temp := outflow_delete_set_KT In m Qn_old).
+        set (In' := outflow_insert_set_KT In_temp m Qn_new).
+        set (Im_temp := inflow_delete_set_KT Im m Qn_old).
+        set (Im' := inflow_insert_set_KT Im_temp m Qn_new).
+
+        iMod ((frac_update γ_en γ_cn γ_bn γ_qn esn' Cn Bn0' Qn0' esn' Cn' Bn0' Qn') 
+             with "[$HnP_frac $HnS_frac]") as "(HnP_frac & HnS_frac)".
+
+        iMod ((frac_update γ_em γ_cm γ_bm γ_qm esm Cm Bm Qm esm Cm' Bm' Qm) 
+             with "[$HnP_fracm $HnS_fracm]") as "(HnP_fracm & HnS_fracm)".
+
+        assert (S ⊆ esn' !!! m) as Sub_S.
+        { intros k Hk. destruct (decide (k ∈ esn' !!! m)); try done.
+          rewrite map_eq_iff in MergeEq *; intros MergeEq.
+          pose proof MergeEq k as MergeEq.
+          unfold merge in MergeEq.
+          rewrite !gmap_imerge_prf in MergeEq.
+          unfold f_merge in MergeEq.
+          destruct (decide (Cn !! k ≠ None)) eqn: Hd; 
+                        rewrite Hd in MergeEq.
+          - destruct (decide (Cn' !! k ≠ None)) eqn: Hd'; 
+                          rewrite Hd' in MergeEq.
+            + pose proof dom_lookup Cn k n1 as H'.
+              pose proof dom_lookup Cn' k n2 as H''.
+              clear -H' H'' S Hk. set_solver.
+            + destruct (decide (k ∈ esn' !!! m)); try done.
+          - destruct (decide (k ∈ esn' !!! m)); try done.
+            clear Hd. apply dec_stable in n1. 
+            apply not_elem_of_dom in n1. 
+            clear -n1 S Hk. set_solver. }
+
+        iAssert (⌜∀ k, Bm !!! k ≤ Bm' !!! k⌝)%I as "%".
+        { admit. }
+        rename H1 into Bm_le_Bm'.
+
+        iAssert (|==> [∗ set] k ∈ KS, own (γ_cirm !!! k)
+                                (● {| max_nat_car := Bm' !!! k |}))%I
+                      with "[HnS_starm]" as ">HnS_starm".
+        { iInduction KS as [| s S'] "IHs" using set_ind_L.
+          - admit.
+          - admit. }
+
+        assert (∀ k t, (k,t) ∈ Qn_new ↔ k ∈ S ∧ t = Cn !!! k) as HQn_new.
+        { admit. }
+        assert (∀ k t, (k,t) ∈ Qn_old ↔ k ∈ S ∧ t = Qn0' !!! k) as HQn_old.
+        { admit. }
+        assert (dom (gset K) S_map = S) as Dom_Smap.
+        { admit. }
+        assert (∀ k, k ∈ S → S_map !! k = Some(Cn !!! k)) as Lookup_Smap.
+        { admit. }
+        assert (∀ k, k ∈ S → Qn' !! k = Cn !! k) as Lookup_Qn'.
+        { admit. }
+        assert (∀ k, k ∉ S → Qn' !! k = Qn0' !! k) as Lookup_Qn'_ne.
+        { admit. }
+        assert (∀ k t, k ∉ S → (k,t) ∉ Qn_old) as HQn_old_ne.
+        { admit. }
+        assert (∀ k t, k ∉ S → (k,t) ∉ Qn_new) as HQn_new_ne.
+        { admit. } 
+        
+        assert (∀ k, k ∈ S → Cn !! k = Cm' !! k) as Lookup_merge.
+        { admit. }
+        
+        assert (∀ k, k ∈ S → Bm !!! k = Qn0' !!! k) as Bm_eq_Qn.
+        { admit. }
+
+        assert (∀ k, k ∈ S → k ∈ inset K Rn n) as S_sub_insetn.
+        { admit. }
+
+        assert (∀ k, k ∈ S → k ∈ inset K Rm m) as S_sub_insetm.
+        { admit. }
+        
+        assert (∀ k, Cn !!! k ≤ T') as Cn_le_T'.
+        { admit. }
+        
+        iDestruct "HnS_oc" as "(%&%&%)".
+        rename H1 into OC1. rename H2 into OC2. rename H3 into OC3.
+        iAssert (outflow_constraints n In' Rn esn' Qn')%I as "HnS_oc".
+        { iPureIntro. split; last split; try done.
+          - intros n' k t. destruct (decide (n' = m)).
+            + subst n'. 
+              assert (outset_KT In' m = 
+                outset_KT In m ∖ Qn_old ∪ Qn_new) as Outset'.
+              { admit. }
+              split.
+              * intros Hout. rewrite Outset' in Hout.
+                rewrite elem_of_union in Hout*; intros Hout.
+                destruct Hout as [Hout | Hout].
+                ** rewrite elem_of_difference in Hout *; intros Hout.
+                   destruct Hout as [Hout1 Hout2].
+                   apply (OC1 m k t) in Hout1.
+                   destruct Hout1 as [H' H''].
+                   assert (Ht := H'').
+                   apply lookup_total_correct in H''.
+                   rewrite <-H'' in Hout2.
+                   assert (k ∉ S) as Hk.
+                   { destruct (decide (k ∈ S)); try done.
+                     assert ((k, Qn0' !!! k) ∈ Qn_old) as HkQn.
+                     apply (HQn_old k (Qn0' !!! k)). 
+                     split; try done. clear -Hout2 HkQn. done. }
+                   split; try done. subst Qn'.
+                   rewrite gmap_lookup_insert_map_ne.
+                   done. by rewrite Dom_Smap.
+                ** apply HQn_new in Hout.
+                   destruct Hout as [Hout1 Hout2].
+                   split. clear -Hout1 Sub_S. set_solver.
+                   subst Qn'. 
+                   rewrite gmap_lookup_insert_map.
+                   rewrite (Lookup_Smap k Hout1).
+                   by rewrite Hout2. by rewrite Dom_Smap.
+              * destruct (decide (k ∈ S)).
+                ** subst Qn'.
+                   rewrite gmap_lookup_insert_map; try done.
+                   rewrite (Lookup_Smap k e). simpl.
+                   intros [H1' H2'].
+                   assert (k ∈ S ∧ t = Cn !!! k) as H''.
+                   split; try done. by inversion H2'.
+                   apply (HQn_new k t) in H''.
+                   clear -H'' Outset'. set_solver.
+                   by rewrite Dom_Smap.
+                ** rewrite (Lookup_Qn'_ne k n0).
+                   intros H'. apply OC1 in H'.
+                   apply (HQn_old_ne k t) in n0.
+                   clear -H' Outset' n0. set_solver.
+            + assert (outset_KT In' n' = outset_KT In n') as Outset'.
+              { admit. }
+              rewrite Outset'.
+              split.
+              * intros Hout. apply OC1 in Hout.
+                destruct Hout as [Hout1 Hout2].
+                assert (k ∉ S) as Hk.
+                { admit. }
+                rewrite (Lookup_Qn'_ne k Hk).
+                split; try done.
+              * intros Hkt.
+                assert (k ∉ S) as Hk.
+                { admit. }
+                rewrite (Lookup_Qn'_ne k Hk) in Hkt.
+                by apply OC1 in Hkt. 
+          - unfold outflow_le_1. intros n' kt. 
+            destruct (decide (n' = m)).
+            * subst n'. subst In'. unfold out, out_map. 
+              unfold outflow_insert_set_KT. simpl.
+              rewrite nzmap_lookup_total_insert.
+              unfold out, out_map.
+              unfold In_temp, outflow_delete_set_KT.
+              simpl. rewrite nzmap_lookup_total_insert.
+              pose proof OC3 m kt as OC3.
+              destruct (decide (kt ∈ Qn_new)).
+              ** rewrite nzmap_lookup_total_increment_set; try done.
+                 destruct (decide (kt ∈ Qn_old)).
+                 *** rewrite nzmap_lookup_total_decrement_set; try done.
+                     clear -OC3. lia.
+                 *** rewrite nzmap_lookup_total_decrement_set_ne; try done.
+                     assert (∀ (x: nat), x ≤ 1 → x = 0 ∨ x = 1) as Hx.
+                     { lia. } apply Hx in OC3.
+                     destruct OC3 as [OC3 | OC3].
+                     rewrite OC3. lia.
+                     assert (kt ∈ outset_KT In m) as Hkt.
+                     { unfold outset_KT, KT_flows.dom_ms.
+                       rewrite nzmap_elem_of_dom_total.
+                       rewrite OC3. unfold ccmunit, ccm_unit; simpl.
+                       by unfold nat_unit. }
+                     destruct kt as [k t].
+                     apply OC1 in Hkt.
+                     destruct Hkt as [_ H'].
+                     apply lookup_total_correct in H'.
+                     rewrite <-H' in n0.
+                     assert ((k, Qn0' !!! k) ∈ Qn_old) as H''.
+                     { apply HQn_old. apply HQn_new in e.
+                       destruct e as [e _]. split; try done. }
+                     clear -H'' n0. done.
+              ** rewrite nzmap_lookup_total_increment_set_ne; try done.
+                 destruct (decide (kt ∈ Qn_old)).
+                 *** rewrite nzmap_lookup_total_decrement_set; try done.
+                     clear -OC3. lia.
+                 *** rewrite nzmap_lookup_total_decrement_set_ne; try done.
+            * subst In'. unfold out, out_map. 
+              unfold outflow_insert_set_KT. simpl.
+              rewrite nzmap_lookup_total_insert_ne; try done.
+              rewrite nzmap_lookup_total_insert_ne; try done.
+              pose proof OC3 n' kt as OC3.
+              by unfold out in OC3. }
+
+        iDestruct "HnS_ocm" as "(%&%&%)".
+        rename H1 into OC1m. rename H2 into OC2m. rename H3 into OC3m.
+
+        iAssert (outflow_constraints m Im' Rm esm Qm)%I as "HnS_ocm".
+        { iPureIntro. split; last split; try done. }
+
+        assert (domm In' = {[n]}) as Domm_In'.
+        { admit. }
+
+        assert (domm Im' = {[m]}) as Domm_Im'.
+        { admit. }
+        
+        iAssert (singleton_interfaces_ghost_state γ_I γ_R n In' Rn
+            ∗ singleton_interfaces_ghost_state γ_I γ_R m Im' Rm)%I 
+                    with "[HnS_si HnS_sim]" as "(HnS_si & HnS_sim)".
+        { iDestruct "HnS_si" as "(HIn & HRn & Domm_In & Domm_Rn)".
+          iDestruct "HnS_sim" as "(HIm & HRm & Domm_Im & Domm_Rm)".
+          iCombine "HIn HIm" as "HInm".
+          assert (Im_temp = inflow_delete_set_KT Im m Qn_old) 
+              as HIm_temp. done.
+          assert (In_temp = outflow_delete_set_KT In m Qn_old)
+              as HIn_temp. done.
+          assert (In' = outflow_insert_set_KT In_temp m Qn_new)
+              as HIn'. done.
+          assert (Im' = inflow_insert_set_KT Im_temp m Qn_new)
+              as HIm'. done.
+          pose proof (flowint_delete_set_eq_KT In In_temp Im Im_temp 
+                  m Qn_old HIn_temp HIm_temp) as HInm_temp.
+          pose proof (flowint_insert_set_eq_KT In_temp In' Im_temp Im' 
+                  m Qn_new HIn' HIm') as HInm'.
+          rewrite HInm' in HInm_temp.
+          iEval (rewrite HInm_temp) in "HInm".
+          iEval (rewrite auth_frag_op) in "HInm".
+          iDestruct "HInm" as "(HIn & HIm)".
+          iFrame. iPureIntro. apply Domm_Im'. }
+        
+        iAssert (⌜φ0 esn' Qn'⌝ ∗ ⌜φ1 Bn0' Cn' Qn'⌝ ∗ ⌜φ2 n Bn0' In'⌝ 
+                  ∗ ⌜φ3 n Bn0' Rn⌝ ∗ ⌜φ4 n Rn⌝ ∗ ⌜φ5 Bn0' Qn'⌝ 
+                  ∗ ⌜φ6 Bn0' T'⌝ ∗ ⌜φ7 n esn' Rn Qn'⌝)%I
+                with "[Hφ]" as "Hφ".
+        { iDestruct "Hφ" as "(%&%&%&%&%&%&%&%)". 
+          rename H1 into Hφ0. rename H2 into Hφ1.
+          rename H3 into Hφ2. rename H4 into Hφ3.
+          rename H5 into Hφ4. rename H6 into Hφ5. 
+          rename H7 into Hφ6. rename H8 into Hφ7.
+          iPureIntro. split; last split; last split; 
+          last split; last split; last split; last split.
+          - unfold φ0. intros k Hnot.
+            assert (k ∉ S) as Hk.
+            { destruct (decide (k ∈ S)); try done.
+              apply Sub_S in e. pose proof Hnot m as Hnot.
+              clear -e Hnot. set_solver. }
+            rewrite (Lookup_Qn'_ne k Hk).
+            apply Hφ0; try done.  
+          - unfold φ1. intros k t'.
+            rewrite map_eq_iff in MergeEq*; intros MergeEq.
+            pose proof MergeEq k as MergeEq.
+            rewrite !gmap_imerge_prf in MergeEq.
+            unfold f_merge in MergeEq. split.
+            + intros HCn'k. destruct (Cn !! k) as [t |] eqn: HCnk.
+              * repeat rewrite decide_True in MergeEq.
+                pose proof Hφ1 k t as [H' _].
+                pose proof H' HCnk as H'.
+                rewrite <-HCn'k, H'. by rewrite <-HCnk.
+                rewrite HCn'k; try done. rewrite HCnk; try done.
+              * pose proof set_of_map_member_ne Cn k HCnk t' as H'.
+                pose proof set_of_map_member Cn' k t' HCn'k as H''.
+                apply Subset_Cn in H''. clear -H' H''.
+                set_solver.
+            + intros HCn'. destruct (Cn !! k) as [t |] eqn: HCnk.
+              * assert (k ∈ S) as Hk.
+                { assert (k ∈ dom (gset K) Cn) as H1'.
+                  rewrite elem_of_dom. rewrite HCnk; by exists t.
+                  assert (k ∉ dom (gset K) Cn') as H2'.
+                  rewrite not_elem_of_dom. done. 
+                  subst S. clear -H1' H2'. set_solver. }
+                rewrite (Lookup_Qn' k Hk).
+                pose proof Hφ1 k t as H'.
+                destruct H' as [H' _].
+                pose proof H' HCnk as H'. 
+                by rewrite H'.
+              * assert (k ∉ S) as Hk.
+                { assert (k ∉ dom (gset K) Cn) as H1'.
+                  rewrite not_elem_of_dom. done. 
+                  subst S. clear -H1'. set_solver. }
+                rewrite (Lookup_Qn'_ne k Hk).
+                pose proof Hφ1 k 0 as H'.
+                destruct H' as [_ H'].
+                by pose proof H' HCnk as H'. 
+          - unfold φ2. try done.
+          - unfold φ3. try done.
+          - try done.
+          - intros k. destruct (decide (k ∈ S)).
+            + rewrite /(Qn' !!! k).
+              unfold finmap_lookup_total. 
+              rewrite (Lookup_Qn' k e).
+              destruct (Cn !! k) as [t |] eqn: HCnk.
+              * pose proof Hφ1 k t as H'.
+                destruct H' as [H' _].
+                pose proof H' HCnk as H'.
+                rewrite lookup_total_alt.
+                by rewrite H'.
+              * by simpl; lia.
+            + rewrite /(Qn' !!! k).
+              rewrite /(Bn0' !!! k). 
+              unfold finmap_lookup_total. 
+              rewrite (Lookup_Qn'_ne k n0).
+              pose proof Hφ5 k as H'.    
+              rewrite /(Qn0' !!! k) in H'.
+              by rewrite /(Bn0' !!! k) in H'. 
+          - try done.
+          - intros k. intros H'. rewrite elem_of_dom.
+            apply Hφ7 in H'. rewrite elem_of_dom in H'*; intros H'.
+            destruct (decide (k ∈ S)).
+            * rewrite (Lookup_Qn' k e).
+              assert (k ∈ dom (gset K) Cn) as H''.
+              { admit. }
+              by rewrite elem_of_dom in H''*; intros H''.
+            * by rewrite (Lookup_Qn'_ne k n0).   }
+                              
+        iAssert (⌜φ0 esm Qm⌝ ∗ ⌜φ1 Bm' Cm' Qm⌝ ∗ ⌜φ2 m Bm' Im'⌝ 
+                  ∗ ⌜φ3 m Bm' Rm⌝ ∗ ⌜φ4 m Rm⌝ ∗ ⌜φ5 Bm' Qm⌝ 
+                  ∗ ⌜φ6 Bm' T'⌝ ∗ ⌜φ7 m esm Rm Qm⌝)%I
+                with "[Hφm]" as "Hφm".
+        { iDestruct "Hφm" as "(%&%&%&%&%&%&%&%)". 
+          rename H1 into Hφ0. rename H2 into Hφ1.
+          rename H3 into Hφ2. rename H4 into Hφ3.
+          rename H5 into Hφ4. rename H6 into Hφ5. 
+          rename H7 into Hφ6. rename H8 into Hφ7. 
+          iPureIntro. split; last split; last split; 
+          last split; last split; last split; last split.
+          - unfold φ0. try done.
+          - unfold φ1. intros k t.
+            rewrite map_eq_iff in MergeEq*; intros MergeEq.
+            pose proof MergeEq k as MergeEq.
+            rewrite !gmap_imerge_prf in MergeEq.
+            unfold f_merge in MergeEq. split.
+            + intros HCm'k. assert (H' := HCm'k). 
+              apply set_of_map_member in H'.
+              apply Subset_Cm in H'.
+              rewrite elem_of_union in H'*; intros H'.
+              destruct H' as [H' | H'].
+              * apply set_of_map_member_rev in H'.
+                subst Bm'. destruct (Cn' !! k) as [t' | ] eqn: HCn'k.
+                ** repeat rewrite decide_True in MergeEq.
+                   assert (t' = t) as Ht.
+                   { rewrite HCn'k H' in MergeEq.
+                     by inversion MergeEq. }
+                   subst t'. 
+                   apply set_of_map_member in H'.
+                   apply set_of_map_member in HCm'k.
+                   apply set_of_map_member in HCn'k.
+                   clear -H' HCm'k  HCn'k Subset_disj. set_solver.
+                   rewrite HCn'k; try done. rewrite H'; try done.
+                ** rewrite decide_True in MergeEq.
+                   rewrite decide_False in MergeEq.
+                   destruct (decide (k ∈ esn' !!! m)).
+                   *** assert (k ∈ S) as Hk.
+                       { admit. }
+                       rewrite gmap_lookup_insert_map.
+                       rewrite (Lookup_Smap k Hk).
+                       rewrite /(Cn !!! k). 
+                       unfold finmap_lookup_total.
+                       rewrite H'; by simpl.
+                       rewrite Dom_Smap. done.
+                   *** rewrite H' in MergeEq.
+                       inversion MergeEq.
+                   *** intros H''. done.
+                   *** rewrite H'. done.
+                * apply set_of_map_member_rev in H'.
+                  pose proof Hφ1 k t as H''.
+                  destruct H'' as [H'' _].
+                  pose proof H'' H' as HBm.
+                  destruct (decide (k ∈ S)).
+                  ** subst Bm'.
+                     rewrite gmap_lookup_insert_map.
+                     rewrite (Lookup_Smap k e).
+                     destruct (Cn !! k) as [t' | ] eqn: HCnk.
+                     *** rewrite decide_True in MergeEq.
+                         destruct (Cn' !! k) as [t'' | ] eqn: HCn'k.
+                         **** assert (k ∉ S) as Hk.
+                              { admit. }
+                              clear -Hk e.
+                              set_solver.
+                         **** rewrite decide_False in MergeEq.
+                              rewrite decide_True in MergeEq.
+                              rewrite HCm'k in MergeEq.
+                              apply lookup_total_correct in MergeEq.
+                              by rewrite MergeEq. by apply Sub_S in e.
+                              rewrite HCn'k. intros Hnone. done.
+                         **** rewrite HCnk; try done.
+                     *** assert (k ∉ S) as Hk.
+                         { admit. }
+                         clear -Hk e. set_solver.
+                     *** by rewrite Dom_Smap.
+                  ** rewrite gmap_lookup_insert_map_ne.
+                     done. by rewrite Dom_Smap.
+            + intros HCm'. assert (Cm !! k = None) as HCm.
+              { admit. }
+              pose proof Hφ1 k 0 as H'.
+              destruct H' as [_ H'].
+              pose proof H' HCm as H'.
+              assert (k ∉ S) as Hk.
+              { destruct (decide (k ∈ S)); try done.
+                subst S. assert (k ∈ dom (gset K) Cn) as H1'.
+                { clear -e. set_solver. }
+                assert (k ∉ dom (gset K) Cn') as H2'.
+                { clear -e. set_solver. }
+                rewrite elem_of_dom in H1'*; intros H1'.
+                rewrite not_elem_of_dom in H2'*; intros H2'.
+                destruct H1' as [t' H1'].
+                rewrite decide_True in MergeEq.
+                rewrite decide_False in MergeEq.
+                rewrite decide_True in MergeEq.
+                rewrite HCm' in MergeEq.
+                rewrite MergeEq in H1'. inversion H1'.
+                by apply Sub_S in e.
+                rewrite H2'. intros ?; try done.
+                rewrite H1'; try done. }
+              subst Bm'. rewrite gmap_lookup_insert_map_ne.
+              done. by rewrite Dom_Smap.
+          - unfold φ2. intros k t Hkt.
+            assert (inset_KT Im' m = 
+                          inset_KT Im m ∖ Qn_old ∪ Qn_new) as Hinset.
+            { admit. }
+            rewrite Hinset in Hkt.
+            rewrite elem_of_union in Hkt*; intros Hkt.
+            destruct Hkt as [Hkt | Hkt].
+            * rewrite elem_of_difference in Hkt*; intros Hkt.
+              destruct Hkt as [Hkt1 Hkt2].
+              apply Hφ2 in Hkt1.
+              destruct (decide (k ∈ S)).
+              ** pose proof Bm_eq_Qn k e as H'.
+                 assert ((k,t) ∈ Qn_old) as H''.
+                 { apply HQn_old. split; try done.
+                   by rewrite H' in Hkt1. }
+                 clear -H'' Hkt2. set_solver.
+              ** rewrite lookup_total_alt. subst Bm'.
+                 rewrite gmap_lookup_insert_map_ne.
+                 by rewrite lookup_total_alt in Hkt1.
+                 by rewrite Dom_Smap.
+            * apply HQn_new in Hkt.
+              destruct Hkt as [Hkt1 Hkt2].
+              rewrite lookup_total_alt.
+              subst Bm'. rewrite gmap_lookup_insert_map.
+              rewrite (Lookup_Smap k Hkt1).
+              by simpl. by rewrite Dom_Smap.
+          - unfold φ3. intros k.
+            destruct (decide (k ∈ S)).
+            + apply S_sub_insetm in e.
+              right. unfold in_inset.
+              by unfold inset in e.
+            + subst Bm'.
+              rewrite gmap_lookup_insert_map_ne.
+              apply Hφ3. by rewrite Dom_Smap.
+          - try done.
+          - intros k. 
+            apply (Nat.le_trans _ (Bm !!! k) _).
+            apply Hφ5. apply Bm_le_Bm'.
+          - intros k. destruct (decide (k ∈ S)).
+            + rewrite /(Bm' !!! k).
+              unfold finmap_lookup_total.
+              subst Bm'.
+              rewrite gmap_lookup_insert_map.
+              rewrite (Lookup_Smap k e). simpl.    
+              apply Cn_le_T'. by rewrite Dom_Smap.
+            + rewrite /(Bm' !!! k).
+              unfold finmap_lookup_total.
+              subst Bm'.
+              rewrite gmap_lookup_insert_map_ne.
+              apply Hφ6. by rewrite Dom_Smap.
+          - try done. }
+
+        assert (set_of_map Cn' ⊆ H) as Cn'_sub_H.
+        { admit. }
+
+        assert (set_of_map Cm' ⊆ H) as Cm'_sub_H.
+        { admit. }
+        
+        iDestruct "Hglob" as "(MCS_auth & HH & Hist & Ht & HI & Out_I & HR 
+            & Out_R & Inf_R & Hf & Hγ & FP_r & Max_ts & domm_IR & domm_Iγ)".
+        iMod (own_update γ_s (● H) 
+             (● H ⋅ ◯ (set_of_map Cn' ⋅ set_of_map Cm')) with "[$HH]") as "HH".
+        { apply (auth_update_alloc _ (H) (set_of_map Cn' ⋅ set_of_map Cm')).
+          apply local_update_discrete. intros mc Valid_H1 H1_eq.
+          split; try done. rewrite /(ε ⋅? mc) in H1_eq.
+          destruct mc. rewrite gset_op_union in H1_eq. 
+          rewrite left_id in H1_eq *; intros H1_eq.
+          rewrite <-H1_eq. 
+          rewrite /(set_of_map Cn' ⋅ set_of_map Cm' ⋅? Some H).
+          rewrite !gset_op_union.
+          clear - Cn'_sub_H Cm'_sub_H. set_solver.
+          rewrite /(set_of_map Cn' ⋅ set_of_map Cm' ⋅? None).
+          rewrite gset_op_union.
+          clear - Cn'_sub_H Cm'_sub_H H1_eq. set_solver. }
+         
+        iClear "HnP_C HnP_Cm".
+        iDestruct "HH" as "(HH & (HnP_C & HnP_Cm))".
+        
+        iAssert (global_state γ_te γ_he γ_s γ_t γ_I γ_R γ_f γ_gh r T' H hγ I R)
+          with "[MCS_auth HH Hist Ht HI Out_I HR Out_R 
+            Inf_R Hf Hγ FP_r Max_ts domm_IR domm_Iγ]" as "Hglob".
+        { iFrame. }     
+        
+        iModIntro.
+        iSplitR "AU HnP_gh HnP_ghm HnP_tm HnP_t node_n node_m 
+                            HnP_C HnP_Cm HnP_frac HnP_fracm".
+        { iNext. iExists T', H, hγ, I, R. iFrame "Hglob".
+          rewrite (big_sepS_delete _ (domm I) n); last by eauto.
+          iSplitL "Hl_n HnS_gh HnS_FP HnS_cl HnS_H HnS_star 
+                       HnS_frac HnS_oc HnS_si Hφ".
+          { iExists true, Cn', Bn0', Qn'. iFrame "Hl_n".
+            iSplitR; try done.
+            iExists γ_en, γ_cn, γ_bn, γ_qn, γ_cirn, esn', In', Rn.
+            iFrame. iFrame "HnS_oc". }
+          rewrite (big_sepS_delete _ (domm I ∖ {[n]}) m); last first.
+          clear -m_neq_n m_in_I. set_solver.
+          iFrame "Hstar'". iExists true, Cm', Bm', Qm.
+          iFrame "Hl_m Hlif_m".
+          iExists γ_em, γ_cm, γ_bm, γ_qm, γ_cirm, esm, Im', Rm.
+          iFrame. rewrite <-PeanoNat.Nat.eqb_neq in m_neq_r.
+          by rewrite m_neq_r. }                            
+        iModIntro.
+        awp_apply (unlockNode_spec_high with "[] [] 
+            [HnP_gh HnP_frac HnP_C HnP_t node_n]"); try done.
+        iExists γ_en, γ_cn, γ_bn, γ_qn, γ_cirn, esn', T.
+        iFrame. iAaccIntro with ""; try eauto with iFrame.
+        iIntros "_"; iModIntro. wp_pures.
+        awp_apply (unlockNode_spec_high with "[] [] 
+            [HnP_ghm HnP_fracm HnP_Cm HnP_tm node_m]"); try done.
+        iExists γ_em, γ_cm, γ_bm, γ_qm, γ_cirm, esm, Tm.
+        iFrame. iAaccIntro with ""; try eauto with iFrame.
+        iIntros "_"; iModIntro. wp_pures.
+        iApply "IH"; try done.
+    + admit.             
+  Admitted.           
   
   Lemma traverse_spec γ_te γ_he γ_s γ_t γ_I γ_R γ_f γ_gh lc r 
                           γ_en γ_cn γ_bn γ_qn γ_cirn n (k: K) t0 t1 :
@@ -767,9 +2376,9 @@ Section multicopy.
     iIntros (t) "(node_n & H)". iDestruct "H" as %Cn_val.
     wp_pures.
     (** Case analysis on whether k in contents of n **)
-    case_eq (bool_decide ((#t = #0))).
+    destruct t as [t |]; last first.
     - (** Case : k not in contents of n **)
-      intros t_eq_0. wp_pures.
+      wp_pures.
       (** Find next node to visit **)
       wp_apply (findNext_spec with "node_n").
       iIntros (b n1) "(node_n & Hif)". 
@@ -784,14 +2393,14 @@ Section multicopy.
         iInv "HInv" as ">H".
         iDestruct "H" as (T' H hγ I R) "(Hglob & Hstar)".
         iAssert (⌜n ∈ domm I⌝)%I as "%". 
-        { iDestruct "Hglob" as "(MCS_auth & HH & Hist & Ht & HI & HR 
-                & Inf_R & Hf & Hγ & FP_r & Max_ts & domm_IR & domm_Iγ)".
+        { iDestruct "Hglob" as "(MCS_auth & HH & Hist & Ht & HI & Out_I & HR 
+            & Out_R & Inf_R & Hf & Hγ & FP_r & Max_ts & domm_IR & domm_Iγ)".
           by iPoseProof (inFP_domm _ _ _ with "[$FP_n] [$Hf]") as "H'". }
         rewrite (big_sepS_delete _ (domm I) n); last by eauto.
         iDestruct "Hstar" as "(H_n & Hstar')".
         iDestruct "H_n" as (bn Cn' Bn' Qn')"(Hl_n & Hlif_n & HnS_n)".
         iDestruct "HnS_n" as (γ_en' γ_cn' γ_bn' γ_qn' γ_cirn' es' In Rn) 
-                      "(HnS_gh & domm_γcir & HnS_frac & HnS_si & HnS_FP 
+                      "(HnS_gh & HnS_frac & HnS_si & HnS_FP 
                                 & HnS_cl & HnS_oc & HnS_H & HnS_star & Hφ)".
         iPoseProof (ghost_heap_sync with "[$HnP_gh] [$HnS_gh]") 
                                   as "(% & % & % & % & %)".
@@ -802,13 +2411,10 @@ Section multicopy.
         iAssert (inFP γ_f n1)%I as "#FP_n1".
         { iApply "HnS_cl". iPureIntro. 
           clear -k_in_es. set_solver. }
-        iAssert (⌜(k, Qn !!! k) ∈ outset_KT In n1⌝)%I as %outflow_n_n1.
-        { iDestruct "HnS_oc" as "(H' & _)".
-          iDestruct "H'" as %H'. iPureIntro. 
-          apply (H' n1 k (Qn !!! k)).
-          repeat split; try done. }
+             
         iAssert (⌜n1 ∈ domm I⌝)%I as %n_in_I.
-        { iDestruct "Hglob" as "(_ & _ & _ & _ & _ & _ &_ & Hf & _)". 
+        { iDestruct "Hglob" as "(MCS_auth & HH & Hist & Ht & HI & Out_I & HR 
+            & Out_R & Inf_R & Hf & Hγ & FP_r & Max_ts & domm_IR & domm_Iγ)".
           by iPoseProof (inFP_domm _ _ _ with "[$FP_n1] [$Hf]") as "H'". }
         iAssert (⌜n ≠ n1⌝)%I as %n_neq_n1.
         { destruct (decide (n = n1)); try done.
@@ -819,67 +2425,12 @@ Section multicopy.
         iDestruct "Hstar'" as "(H_n1 & Hstar'')".
         iDestruct "H_n1" as (bn1 Cn1 Bn1 Qn1)"(Hl_n1 & Hlif_n1 & HnS_n1)".
         iDestruct "HnS_n1" as (γ_en1 γ_cn1 γ_bn1 γ_qn1 γ_cirn1 es1 In1 Rn1) 
-                  "(HnS_gh1 & domm_γcir1 & HnS_frac1 & HnS_si1 & HnS_FP1 
+                  "(HnS_gh1 & HnS_frac1 & HnS_si1 & HnS_FP1 
                        & HnS_cl1 & HnS_oc1 & HnS_H1 & HnS_star1 & Hφ1)".
-        iAssert (⌜(k, Qn !!! k) ∈ inset_KT In1 n1⌝)%I as %inflow_n1.
-        { iDestruct "HnS_si" as "(H'&_)".
-          iDestruct "HnS_si1" as "(H1'&_&%&_)".
-          rename H1 into Domm_In1.
-          assert (n1 ∈ domm In1) as H''. 
-          { clear -Domm_In1. set_solver. }
-          iCombine "H'" "H1'" as "H'".
-          iPoseProof (own_valid with "[$H']") as "%".
-          rename H1 into Valid_InIn1.
-          rewrite auth_frag_valid in Valid_InIn1 *; intros Valid_InIn1.
-          pose proof intComp_unfold_inf_2 In In1 Valid_InIn1 n1 H''.
-          rename H1 into H'. unfold ccmop, ccm_op in H'.
-          simpl in H'. unfold lift_op in H'.
-          iPureIntro. rewrite nzmap_eq in H' *; intros H'.
-          pose proof H' (k, Qn !!! k) as H'.
-          rewrite nzmap_lookup_merge in H'.
-          unfold ccmop, ccm_op in H'. simpl in H'.
-          unfold nat_op in H'.
-          assert (1 ≤ out In n1 !1 (k, Qn !!! k)) as Hout.
-          { unfold outset_KT, KT_flows.dom_ms in outflow_n_n1.
-            rewrite nzmap_elem_of_dom_total in outflow_n_n1 *; 
-            intros outflow_n_n1.
-            unfold ccmunit, ccm_unit in outflow_n_n1.
-            simpl in outflow_n_n1. unfold nat_unit in outflow_n_n1.
-            clear - outflow_n_n1. lia. }
-          assert (1 ≤ inf In1 n1 !1 (k, Qn !!! k)) as Hin.
-          { clear -H' Hout. 
-            assert (∀ (x y z: nat), 1 ≤ y → x = z + y → 1 ≤ x) as H''.
-            lia. by pose proof H'' _ _ _ Hout H'. }
-          unfold inset_KT. rewrite nzmap_elem_of_dom_total.
-          unfold ccmunit, ccm_unit. simpl. unfold nat_unit.
-          clear -Hin. lia. }
-        iAssert (⌜n1 ≠ r⌝)%I as %n1_neq_r.
-        { iDestruct "Hφ" as "(_ & _ & _ & _ & _ & %)".
-          rename H1 into Hφ5. iPureIntro.
-          destruct (decide (n1 = r)); try done.
-          unfold φ5 in Hφ5. rewrite <-e in Hφ5.
-          clear -Hφ5 k_in_es. set_solver. }      
-        iAssert (⌜Bn1 !!! k = Qn !!! k⌝)%I as %Bn1_eq_Bn.
-        { iDestruct "Hφ1" as "(_ & _ & % & _)". 
-          rename H1 into Hφ2.
-          by pose proof Hφ2 k (Qn !!! k) n1_neq_r inflow_n1. } 
+
         iEval (rewrite (big_sepS_elem_of_acc (_) (KS) k); 
                               last by eauto) in "HnS_star".
         iDestruct "HnS_star" as "(Hcirk_n & HnS_star')".
-        iAssert (⌜t1 ≤ Bn !!! k⌝)%I as %lb_t1.
-        { iPoseProof (own_valid_2 with "[$Hcirk_n] [$Hlb]") as "%".
-          rename H1 into Valid_Bnt.
-          apply auth_both_valid_discrete in Valid_Bnt.
-          destruct Valid_Bnt as [H' _].
-          apply max_nat_included in H'.
-          simpl in H'. by iPureIntro. }
-        iAssert (⌜Bn !!! k = Qn !!! k⌝)%I as %Bn_eq_Qn.
-        { iDestruct "Hφ" as "(_ & % & _)". rename H1 into Hφ1.
-          apply bool_decide_eq_true in t_eq_0.
-          inversion t_eq_0 as [H''].
-          pose proof Hφ1 k as [_ H'].
-          iPureIntro. apply H'. rewrite Cn_val.
-          clear -H''. lia. }  
         iEval (rewrite (big_sepS_elem_of_acc (_) (KS) k);
                                      last by eauto) in "HnS_star1".
         iDestruct "HnS_star1" as "(Hcirk_n1 & HnS_star1')".
@@ -890,6 +2441,78 @@ Section multicopy.
                               (MaxNat (Bn1 !!! k))).
           apply max_nat_local_update. 
           simpl. lia. } { iFrame. }
+
+        iAssert (⌜t0 ≤ Bn1 !!! k⌝)%I as "%".
+        { iAssert (⌜t1 ≤ Bn !!! k⌝)%I as %lb_t1.
+          { iPoseProof (own_valid_2 with "[$Hcirk_n] [$Hlb]") as "%".
+            rename H1 into Valid_Bnt.
+            apply auth_both_valid_discrete in Valid_Bnt.
+            destruct Valid_Bnt as [H' _].
+            apply max_nat_included in H'.
+            simpl in H'. by iPureIntro. }
+          destruct (Qn !! k) as [tq | ] eqn: Hqn.
+          - iAssert (⌜(k, Qn !!! k) ∈ outset_KT In n1⌝)%I as %outflow_n_n1.
+            { iDestruct "HnS_oc" as "(H' & _)".
+              iDestruct "H'" as %H'. iPureIntro.    
+              apply (H' n1 k (Qn !!! k)).
+              unfold outflow_constraint_I in H'.
+              repeat split; try done. 
+              rewrite lookup_total_alt. 
+              rewrite Hqn. by simpl. }
+            iAssert (⌜(k, Qn !!! k) ∈ inset_KT In1 n1⌝)%I as %inflow_n1.
+            { iDestruct "HnS_si" as "(H'&_)".
+              iDestruct "HnS_si1" as "(H1'&_&%&_)".
+              rename H1 into Domm_In1.
+              assert (n1 ∈ domm In1) as H''. 
+              { clear -Domm_In1. set_solver. }
+              iCombine "H'" "H1'" as "H'".
+              iPoseProof (own_valid with "[$H']") as "%".
+              rename H1 into Valid_InIn1.
+              rewrite auth_frag_valid in Valid_InIn1 *; intros Valid_InIn1.
+              pose proof intComp_unfold_inf_2 In In1 Valid_InIn1 n1 H''.
+              rename H1 into H'. unfold ccmop, ccm_op in H'.
+              simpl in H'. unfold lift_op in H'.
+              iPureIntro. rewrite nzmap_eq in H' *; intros H'.
+              pose proof H' (k, Qn !!! k) as H'.
+              rewrite nzmap_lookup_merge in H'.
+              unfold ccmop, ccm_op in H'. simpl in H'.
+              unfold nat_op in H'.
+              assert (1 ≤ out In n1 !1 (k, Qn !!! k)) as Hout.
+              { unfold outset_KT, KT_flows.dom_ms in outflow_n_n1.
+                rewrite nzmap_elem_of_dom_total in outflow_n_n1 *; 
+                intros outflow_n_n1.
+                unfold ccmunit, ccm_unit in outflow_n_n1.
+                simpl in outflow_n_n1. unfold nat_unit in outflow_n_n1.
+                clear - outflow_n_n1. lia. }
+              assert (1 ≤ inf In1 n1 !1 (k, Qn !!! k)) as Hin.
+              { clear -H' Hout. 
+                assert (∀ (x y z: nat), 1 ≤ y → x = z + y → 1 ≤ x) as H''.
+                lia. by pose proof H'' _ _ _ Hout H'. }
+              unfold inset_KT. rewrite nzmap_elem_of_dom_total.
+              unfold ccmunit, ccm_unit. simpl. unfold nat_unit.
+              clear -Hin. lia. }
+            iAssert (⌜Bn1 !!! k = Qn !!! k⌝)%I as %Bn1_eq_Bn.
+            { iDestruct "Hφ1" as "(_ & _& % & _)". 
+              rename H1 into Hφ2. pose proof Hφ2 k (Qn !!! k) inflow_n1 as H'.
+              iPureIntro. done. } 
+            iAssert (⌜Bn !!! k = Qn !!! k⌝)%I as %Bn_eq_Qn.
+            { iDestruct "Hφ" as "(_ & % & _)". rename H1 into Hφ1.
+              pose proof Hφ1 k as [_ H'].
+              iPureIntro. pose proof H' Cn_val as H'. 
+              rewrite /(Bn !!! k). unfold finmap_lookup_total.
+              by rewrite H'.  } 
+            iPureIntro. rewrite Bn1_eq_Bn.
+            rewrite <-Bn_eq_Qn. clear -lb_t1 t0_le_t1.
+            apply (Nat.le_trans _ t1 _); try done.
+          - iDestruct "Hφ" as "(_ & % & _)".
+            rename H1 into Hφ1. apply Hφ1 in Cn_val.
+            rewrite <-Cn_val in Hqn.
+            rewrite lookup_total_alt in lb_t1.
+            rewrite Hqn in lb_t1.
+            simpl in lb_t1. iPureIntro.
+            clear -lb_t1 t0_le_t1. lia.
+            try done. }
+ 
         iAssert (own γ_gh (◯ {[n1 := 
                       ghost_loc γ_en1 γ_cn1 γ_bn1 γ_qn1 γ_cirn1]}))%I
                             with "HnS_gh1" as "#Hgh1".  
@@ -898,7 +2521,7 @@ Section multicopy.
         iExists T', H, hγ, I, R. iFrame "Hglob".
         rewrite (big_sepS_delete _ (domm I) n); last by eauto.
         rewrite (big_sepS_delete _ (domm I ∖ {[n]}) n1); last set_solver.
-        iFrame "Hstar''". iSplitL "Hl_n Hlif_n HnS_gh domm_γcir HnS_frac 
+        iFrame "Hstar''". iSplitL "Hl_n Hlif_n HnS_gh HnS_frac 
                     HnS_si HnS_FP HnS_cl HnS_oc HnS_H Hcirk_n HnS_star' Hφ".
         iExists bn, Cn, Bn, Qn. iFrame "Hl_n Hlif_n".
         iExists γ_en, γ_cn, γ_bn, γ_qn, γ_cirn, es, In, Rn.
@@ -915,10 +2538,7 @@ Section multicopy.
         iAaccIntro with ""; try eauto with iFrame.
         iIntros "_". iModIntro. wp_pures.
         (** Apply IH on node n' **)
-        iApply "IH"; try done. iPureIntro.
-        rewrite Bn1_eq_Bn. rewrite <-Bn_eq_Qn.
-        clear -lb_t1 t0_le_t1.
-        apply (Nat.le_trans t0 t1 _); try done.
+        iApply "IH"; try done. 
       + (** Case : no next node from n **)
         wp_pures. iDestruct "Hif" as %Not_in_es.
         iApply fupd_wp. 
@@ -928,14 +2548,14 @@ Section multicopy.
         iInv "HInv" as ">H".
         iDestruct "H" as (T' H hγ I R) "(Hglob & Hstar)".
         iAssert (⌜n ∈ domm I⌝)%I as "%". 
-        { iDestruct "Hglob" as "(MCS_auth & HH & Hist & Ht & HI & HR 
-                & Inf_R & Hf & Hγ & FP_r & Max_ts & domm_IR & domm_Iγ)".
+        { iDestruct "Hglob" as "(MCS_auth & HH & Hist & Ht & HI & Out_I & HR 
+            & Out_R & Inf_R & Hf & Hγ & FP_r & Max_ts & domm_IR & domm_Iγ)".
           by iPoseProof (inFP_domm _ _ _ with "[$FP_n] [$Hf]") as "H'". }
         rewrite (big_sepS_delete _ (domm I) n); last by eauto.
         iDestruct "Hstar" as "(H_n & Hstar')".
         iDestruct "H_n" as (bn Cn' Bn' Qn')"(Hl_n & Hlif_n & HnS_n)".
         iDestruct "HnS_n" as (γ_en' γ_cn' γ_bn' γ_qn' γ_cirn' es' In Rn) 
-                      "(HnS_gh & domm_γcir & HnS_frac & HnS_si & HnS_FP 
+                      "(HnS_gh & HnS_frac & HnS_si & HnS_FP 
                                 & HnS_cl & HnS_oc & HnS_H & HnS_star & Hφ)".
         iPoseProof (ghost_heap_sync with "[$HnP_gh] [$HnS_gh]") 
                                   as "(% & % & % & % & %)".
@@ -949,12 +2569,10 @@ Section multicopy.
           iDestruct "Hφ1" as %Hφ1.
           pose proof Hφ0 k Not_in_es as Hφ0.
           pose proof Hφ1 k as [_ H'].
-          rewrite Hφ0 in H'. 
-          iPureIntro. apply H'.
-          apply bool_decide_eq_true in t_eq_0.
-          inversion t_eq_0 as [H''].
-          rewrite Cn_val.
-          clear -H''. lia. }          
+          pose proof H' Cn_val as H'. 
+          iPureIntro.
+          rewrite lookup_total_alt.
+          rewrite H' Hφ0. by simpl. }          
         iEval (rewrite (big_sepS_elem_of_acc (_) (KS) k); last by eauto) 
                                                        in "HnS_star".
         iDestruct "HnS_star" as "(Hcirk_n & HnS_star')".
@@ -971,15 +2589,15 @@ Section multicopy.
         (** Linearization **)  
         iMod "AU" as (t' H') "[MCS [_ Hclose]]". 
         iAssert (⌜H' = H⌝)%I as %H1. 
-        { iDestruct "Hglob" as "(MCS_auth & HH & Hist & Ht & HI & HR & Hf 
-                & Hγ & FP_r & Max_ts & domm_IR & domm_Iγ)".
+        { iDestruct "Hglob" as "(MCS_auth & HH & Hist & Ht & HI & Out_I & HR 
+            & Out_R & Inf_R & Hf & Hγ & FP_r & Max_ts & domm_IR & domm_Iγ)".
           iPoseProof ((auth_agree' γ_he) with "[MCS_auth] [MCS]") as "%".
           unfold MCS_auth. by iDestruct "MCS_auth" as "(_ & H'')".
           by iDestruct "MCS" as "(_ & H')".
           by iPureIntro. } subst H'.
         iAssert (⌜(k,0) ∈ H⌝)%I as "%". 
-        { iDestruct "Hglob" as "(MCS_auth & HH & Hist & Ht & HI & HR 
-                & Inf_R & Hf & Hγ & FP_r & Max_ts & domm_IR & domm_Iγ)".
+        { iDestruct "Hglob" as "(MCS_auth & HH & Hist & Ht & HI & Out_I & HR 
+            & Out_R & Inf_R & Hf & Hγ & FP_r & Max_ts & domm_IR & domm_Iγ)".
           iDestruct "Hist" as %Hist. iPureIntro. 
           by pose proof Hist k k_in_KS as Hist. }
         rename H1 into k0_in_H.  
@@ -1001,7 +2619,7 @@ Section multicopy.
         iAaccIntro with ""; try eauto with iFrame.
         iIntros "_". iModIntro. iIntros "HΦ". by wp_pures.
     - (** Case : k in contents of n **)
-      intros t_eq_0. wp_pures.                                         
+      wp_pures.                                         
       iApply fupd_wp. 
       (** Linearization Point: key k has been found. Open 
           invariant to obtain resources required to 
@@ -1009,14 +2627,14 @@ Section multicopy.
       iInv "HInv" as ">H".
       iDestruct "H" as (T' H hγ I R) "(Hglob & Hstar)".
       iAssert (⌜n ∈ domm I⌝)%I as "%". 
-      { iDestruct "Hglob" as "(MCS_auth & HH & Hist & Ht & HI & HR 
-              & Inf_R & Hf & Hγ & FP_r & Max_ts & domm_IR & domm_Iγ)".
+      { iDestruct "Hglob" as "(MCS_auth & HH & Hist & Ht & HI & Out_I & HR 
+            & Out_R & Inf_R & Hf & Hγ & FP_r & Max_ts & domm_IR & domm_Iγ)".
         by iPoseProof (inFP_domm _ _ _ with "[$FP_n] [$Hf]") as "H'". }
       rewrite (big_sepS_delete _ (domm I) n); last by eauto.
       iDestruct "Hstar" as "(H_n & Hstar')".
       iDestruct "H_n" as (bn Cn' Bn' Qn')"(Hl_n & Hlif_n & HnS_n)".
       iDestruct "HnS_n" as (γ_en' γ_cn' γ_bn' γ_qn' γ_cirn' es' In Rn) 
-                    "(HnS_gh & domm_γcir & HnS_frac & HnS_si & HnS_FP 
+                    "(HnS_gh & HnS_frac & HnS_si & HnS_FP 
                               & HnS_cl & HnS_oc & HnS_H & HnS_star & Hφ)".
       iPoseProof (ghost_heap_sync with "[$HnP_gh] [$HnS_gh]") 
                                 as "(% & % & % & % & %)".
@@ -1037,17 +2655,14 @@ Section multicopy.
       iAssert (⌜Bn !!! k = Cn !!! k⌝)%I as %Bn_eq_Cn.
       { iDestruct "Hφ" as "(_ & Hφ1 & _)".
         iDestruct "Hφ1" as %Hφ1.
-        pose proof Hφ1 k as [H' _].
-        iPureIntro. apply H'.
-        apply bool_decide_eq_false in t_eq_0.
-        rewrite Cn_val.
-        clear -t_eq_0. apply neq_0_lt. 
-        unfold not. intros H'. 
-        apply t_eq_0. apply f_equal. 
-        rewrite <-H'. done. }          
+        pose proof Hφ1 k t as [H' _].
+        iPureIntro.
+        rewrite !lookup_total_alt.
+        pose proof H' Cn_val as H'.
+        by rewrite Cn_val H'. }          
       iAssert (⌜set_of_map Cn ⊆ H⌝)%I as %Cn_Sub_H.
-      { iDestruct "Hglob" as "(MCS_auth & HH & Hist & Ht & HI & HR 
-              & Inf_R & Hf & Hγ & FP_r & Max_ts & domm_IR & domm_Iγ)".
+      { iDestruct "Hglob" as "(MCS_auth & HH & Hist & Ht & HI & Out_I & HR 
+            & Out_R & Inf_R & Hf & Hγ & FP_r & Max_ts & domm_IR & domm_Iγ)".
         iPoseProof ((auth_own_incl γ_s H _) with "[$HH $HnP_C]") as "%".
         rename H1 into H'. by apply gset_included in H'. }  
       iAssert (⌜(k,t) ∈ set_of_map Cn⌝)%I as %kt_in_Cn.
@@ -1056,24 +2671,23 @@ Section multicopy.
         unfold finmap_lookup_total, inhabitant in Cn_val.
         simpl in Cn_val. 
         destruct (Cn !! k) as [cnk | ] eqn: Hcnk.
-        - rewrite Hcnk. apply f_equal. 
-          by simpl in Cn_val.
-        - simpl in Cn_val.
-          apply bool_decide_eq_false_1 in t_eq_0.
-          exfalso. apply t_eq_0. replace t. try done. }
+        - rewrite Hcnk. apply f_equal.
+          by inversion Cn_val. 
+        - try done.  }
       (** Linearization **)      
       iMod "AU" as (t' H') "[MCS [_ Hclose]]". 
       iSpecialize ("Hclose" $! t).
       iAssert (⌜H' = H⌝)%I as %H1. 
-      { iDestruct "Hglob" as "(MCS_auth & HH & Hist & Ht & HI & HR 
-              & Inf_R & Hf & Hγ & FP_r & Max_ts & domm_IR & domm_Iγ)".
+      { iDestruct "Hglob" as "(MCS_auth & HH & Hist & Ht & HI & Out_I & HR 
+            & Out_R & Inf_R & Hf & Hγ & FP_r & Max_ts & domm_IR & domm_Iγ)".
         iPoseProof ((auth_agree' γ_he) with "[MCS_auth] [MCS]") as "%".
         unfold MCS_auth. by iDestruct "MCS_auth" as "(_ & H'')".
         by iDestruct "MCS" as "(_ & H')".
         by iPureIntro. } replace H'.
       iMod ("Hclose" with "[MCS]") as "HΦ". iFrame. 
       iPureIntro. split. set_solver. rewrite Bn_eq_Cn in lb_t1.
-      rewrite Cn_val in lb_t1. lia.
+      rewrite lookup_total_alt in lb_t1.
+      rewrite Cn_val in lb_t1. simpl in lb_t1. lia.
       (** Closing the invariant **)
       iModIntro. iSplitR "node_n HnP_gh HnP_frac HnP_C HnP_t HΦ".
       iNext. iExists T', H, hγ, I, R. iFrame "Hglob".
@@ -1089,7 +2703,8 @@ Section multicopy.
       iExists γ_en, γ_cn, γ_bn, γ_qn, γ_cirn, es, T. iFrame.
       iAaccIntro with ""; try eauto with iFrame.
       iIntros "_". iModIntro. iIntros "HΦ". by wp_pures.
-  Qed.  
+      Unshelve. try done. try done.
+  Qed.
 
   Lemma upsert_spec γ_te γ_he γ_s γ_t γ_I γ_R γ_f γ_gh lc r (k: K) :
     ⊢ ⌜k ∈ KS⌝ -∗ 
@@ -1105,8 +2720,8 @@ Section multicopy.
     (** Open invariant to establish root node in footprint **)
     iInv "HInv" as ">H".
     iDestruct "H" as (T0 H0 hγ0 I0 R0) "(Hglob & Hstar)".
-    iDestruct "Hglob" as "(MCS_auth & HH & Hist & Ht & HI & HR & 
-              Inf_R & Hf & Hγ & #FP_r & Max_ts & domm_IR & domm_Iγ)".
+    iDestruct "Hglob" as "(MCS_auth & HH & Hist & Ht & HI & Out_I & HR 
+            & Out_R & Inf_R & Hf & Hγ & #FP_r & Max_ts & domm_IR & domm_Iγ)".
     iModIntro. iSplitR "AU". iNext. 
     iExists T0, H0, hγ0, I0, R0. iFrame "∗ #". iModIntro.
     (** Lock the node r **)
@@ -1135,8 +2750,8 @@ Section multicopy.
       (** Linearization Point: open invariant and update the resources **)
       awp_apply (incrementClock_spec γ_t lc T). iInv "HInv" as ">H". 
       iDestruct "H" as (T1 H1 hγ1 I1 R1) "(Hglob & Hstar)".
-      iDestruct "Hglob" as "(MCS_auth & HH & Hist & Ht & HI & HR 
-                & Inf_R & Hf & Hγ & _ & Max_ts & domm_IR & domm_Iγ)".
+      iDestruct "Hglob" as "(MCS_auth & HH & Hist & Ht & HI & Out_I & HR 
+            & Out_R & Inf_R & Hf & Hγ & _ & Max_ts & domm_IR & domm_Iγ)".
       iDestruct "Hif" as %HCr. wp_pures.
       iAssert (⌜T = T1⌝)%I as %HT. 
       { iDestruct "HnP_t" as "(HnP_t & Hc)".
@@ -1198,10 +2813,11 @@ Section multicopy.
         clear - H' Cr_sub_H1 Cr_sub_H1'. set_solver.
         exfalso. clear -H1_eq. set_solver. }
       (** Re-establish history_init **)   
-      iAssert (history_init (H1 ∪ {[(k, T)]})) with "[Hist]" as "Hist".
+      iAssert (⌜history_init (H1 ∪ {[(k, T)]})⌝)%I with "[Hist]" as "Hist".
       { iDestruct "Hist" as %Hist.
         unfold history_init. iPureIntro.
-        clear -Hist. set_solver. }  
+        clear -Hist k_in_KS. intros k' Hk'.
+        pose proof Hist k' Hk' as H'. set_solver. }  
       iDestruct "HnP_C" as "_".  
       iDestruct "HH" as "(HH & HnP_C)".   
       iAssert (⌜r ∈ domm I1⌝)%I as %r_in_I.
@@ -1216,7 +2832,7 @@ Section multicopy.
         iPoseProof ((node_sep_star r r) with "[$]") as "%".
         contradiction. } replace br.
       iDestruct "HnS_r" as (γ_er' γ_cr' γ_br' γ_qr' γ_cirr' es' Ir Rr) 
-                    "(HnS_gh & domm_γcir & HnS_frac & HnS_si & HnS_FP 
+                    "(HnS_gh & HnS_frac & HnS_si & HnS_FP 
                               & HnS_cl & HnS_oc & HnS_if & HnS_star & Hφ)".
       iPoseProof (ghost_heap_sync with "[$HnP_gh] [$HnS_gh]") 
                                 as "(% & % & % & % & %)".
@@ -1228,7 +2844,8 @@ Section multicopy.
       set (Br' := <[k := T]>Br).
       assert (Br' = <[k := T]>Br) as HBr'. try done.
       iEval (rewrite <-beq_nat_refl) in "HnS_if".
-      iDestruct "HnS_if" as %Br_eq_H1.
+      iDestruct "HnS_if" as "(% & %)". 
+      rename H into Br_eq_H1. rename H2 into Infz_Ir.
       iAssert (⌜Br' = map_of_set (H1 ∪ {[(k, T)]})⌝)%I as %Br'_eq_H1.
       { iPureIntro.
         apply map_of_set_insert_eq; try done.
@@ -1238,7 +2855,7 @@ Section multicopy.
       iEval (rewrite (big_sepS_delete (_) (KS) k); last by eauto) in "HnS_star".
       iDestruct "HnS_star" as "(Hk & HnS_star')".
       iAssert (⌜Br !!! k ≤ T⌝)%I as %Br_le_T. 
-      { iDestruct "Hφ" as "(_&_&_&_&_&_&%)".
+      { iDestruct "Hφ" as "(_&_&_&_&_&_&%&_)".
         iPureIntro. rename H into H'.
         by pose proof H' k. }
       iMod (own_update (γ_cirr !!! k) (● (MaxNat (Br !!! k))) 
@@ -1267,7 +2884,7 @@ Section multicopy.
         { apply lookup_total_insert_ne; try done. } 
         by iEval (rewrite H'').
         done. }
-      iMod ((frac_update γ_er γ_cr γ_br γ_qr r es Cr Br Qr es Cr' Br' Qr) 
+      iMod ((frac_update γ_er γ_cr γ_br γ_qr es Cr Br Qr es Cr' Br' Qr) 
                   with "[$HnP_frac $HnS_frac]") as "(HnP_frac & HnS_frac)".
       iDestruct "Inf_R" as %Inf_R.
       iPoseProof ((auth_own_incl γ_R R1 Rr) with "[HR HnS_si]")
@@ -1280,33 +2897,42 @@ Section multicopy.
       iAssert (⌜domm Rr = {[r]}⌝)%I as "%".
       { by iDestruct "HnS_si" as "(_&_&_&H')". }
       rename H into Domm_Rr.
-      iAssert (⌜φ0 es Qr⌝ ∗ ⌜φ1 Br' Cr' Qr⌝ ∗ ⌜φ2 r r Br' Ir⌝ 
-        ∗ ⌜φ3 r Br' Rr⌝ ∗ ⌜φ4 r Rr⌝ ∗ ⌜φ5 es r⌝ ∗ ⌜φ6 Br' (T+1)⌝)%I 
+      iAssert (⌜φ0 es Qr⌝ ∗ ⌜φ1 Br' Cr' Qr⌝ ∗ ⌜φ2 r Br' Ir⌝ 
+        ∗ ⌜φ3 r Br' Rr⌝ ∗ ⌜φ4 r Rr⌝ ∗ ⌜φ5 Br' Qr⌝ 
+        ∗ ⌜φ6 Br' (T+1)⌝ ∗ ⌜φ7 r es Rr Qr⌝)%I 
             with "[Hφ]" as "Hφ".
       { iDestruct "Hφ" as %Hφ. 
-        destruct Hφ as [Hφ0 [Hφ1 [Hφ2 [Hφ3 [Hφ4 [Hφ5 Hφ6]]]]]].
+        destruct Hφ as [Hφ0 [Hφ1 [Hφ2 [Hφ3 [Hφ4 [Hφ5 [Hφ6 Hφ7]]]]]]].
         iPureIntro. repeat split; try done.
         - destruct (decide (k0 = k)).
           + subst k0. subst Cr' Br'.
-            rewrite !lookup_total_insert. try done.
+            rewrite !lookup_insert. try done.
           + subst Cr' Br'. 
-            rewrite !lookup_total_insert_ne; try done.
+            rewrite !lookup_insert_ne; try done.
             by pose proof Hφ1 k0 as [H' _].
         - destruct (decide (k0 = k)).
           + subst k0. subst Cr' Br'.
-            rewrite !lookup_total_insert.
+            rewrite !lookup_insert.
             destruct Max_tsH1 as [_ H'].
-            intros H''; clear -H' H''; lia.
-          + subst Cr' Br'. 
-            rewrite !lookup_total_insert_ne; try done.
-            by pose proof Hφ1 k0 as [_ H'].
-        - intros k' t' Hr. clear -Hr. done.
+            intros H''; inversion H''.
+          + (* This is the cause of later admit *)
+            subst Cr' Br'. 
+            rewrite !lookup_insert_ne; try done.
+            pose proof Hφ1 k0 as [_ H']. done.
+        - intros k' t' Hins.
+          pose proof Infz_Ir r as Infz_Ir.
+          rewrite Infz_Ir in Hins.
+          exfalso. clear -Hins. set_solver.
         - intros k'. right.
           apply (inset_monotone R1 Rr Ro); try done.
           by rewrite <-auth_auth_valid.
           pose proof Inf_R r k' as Inf_R.
           by rewrite <-beq_nat_refl in Inf_R.
           rewrite Domm_Rr. clear. set_solver.
+        - intros k'. subst Br'. destruct (decide (k' = k)).
+          + subst k'. rewrite lookup_total_insert.
+            apply (Nat.le_trans _ (Br !!! k) _); try done.
+          + rewrite lookup_total_insert_ne; try done.    
         - intros k'. destruct (decide (k' = k)).
           + subst k' Br'. rewrite lookup_total_insert; lia.
           + subst Br'. rewrite lookup_total_insert_ne; try done.
@@ -1363,7 +2989,7 @@ Section multicopy.
         iDestruct "HnS" as (γ_e γ_c γ_b γ_q γ_cir esy Iy Ry)
                     "(HnS_gh & domm_γcir & HnS_frac & HnS_si & HnS_FP 
                               & HnS_cl & HnS_oc & HnS_if & HnS_star 
-                              & Hφ0 & Hφ1 & Hφ2 & Hφ3 & Hφ4 & Hφ5 & Hφ6)".
+                              & Hφ0 & Hφ1 & Hφ2 & Hφ3 & Hφ4 & Hφ6 & Hφ7)".
         iExists γ_e, γ_c, γ_b, γ_q, γ_cir, esy, Iy, Ry. iFrame.
         iDestruct "Hφ6" as %Hφ6. 
         assert (y =? r = false) as Hyr by (rewrite beq_nat_false_iff; done).
@@ -1376,7 +3002,10 @@ Section multicopy.
         [HnP_gh HnP_t HnP_C HnP_frac node_r]") without "HΦ"; try done. 
       iExists γ_er, γ_cr, γ_br, γ_qr, γ_cirr, es, (T + 1).
       iFrame. by iEval (rewrite <-beq_nat_refl).
-      iAaccIntro with ""; try eauto with iFrame.
+      iAaccIntro with ""; try done.
+      iIntros "_". iModIntro; iIntros "HΦ"; try done.
+      Unshelve. try done.
   Qed.      
+
 
     
